\documentclass[11pt]{article}
\usepackage{homework}

\classname{444}
\homeworknum{3}



\begin{document}

\input{definitions}
\input{probdefs}


\state{Renormalization of Yukawa theory (P\&S 10.2)}{
	Consider the pseudoscalar Yukawa Lagrangian,
	\eqn{given1}{
		\cL = \frac{1}{2} (\ptsm \phi)^2 - \frac{1}{2} m^2 \phi^2 + \psib (i \ptsl - M) \psi - i g \psib \gamt \psi \phi,
	}
	where $\phi$ is a real scalar field and $\psi$ is a Dirac fermion.  Notice that this Lagrangian is invariant under the parity transformation $\psi(t, \vx) \to \gamo \psi(zt, -\vx)$, $\phi(t, \vx) \to -\phi(t, -\vx)$, in which the field $\phi$ carries odd parity.
}

\prob{ \label{1a}
	Determine the superficially divergent amplitudes and work out the Feynman rules for renormalized perturbation theory for this Lagrangian.  Include all necessary counterterm vertices.  Show that the theory contains a superficially divergent $4 \phi$ amplitude.  This means that the theory cannot be renormalized unless one includes a scalar self-interaction,
	\eqn{given1a}{
		\del\cL = \frac{\lam}{4!} \phi^4,
	}
	and a counterterm of the same form.  It is of course possible to set the renormalized value of this coupling to zero, but that is not a natural choice, since the counterterm will still be nonzero.  Are any further interactions required?
}

\sol{
	We write Eq.~\refeq{given1} explicitly in terms of the bare masses $\mo, \Mo$ and the bare coupling constant $\go$:
	\eqn{newlagr}{
		\cL = \frac{1}{2} (\ptsm \phi)^2 - \frac{1}{2} \mo^2 \phi^2 + \psib (i \ptsl - \Mo) \psi - i \go \psib \gamt \psi \phi,
	}
	The Feynman rules for a pseudoscalar Yukawa theory are~\cite[pp.~24--25]{FR} \\[-5ex]
	\al{
		\centergraphics{diag/scalar_prop} &= \frac{i}{q^2 - \mo^2 + i \eps} &
		\centergraphics{diag/fermion_prop} &= \frac{i (\psl + \Mo)}{p^2 - \Mo^2 + i \eps} \\[-7ex]
	}
	\eq{
		\centergraphics{diag/scalar_fermion_vertex} = \go \gamt
	}
	These Feynman rules are similar enough to those for QED; that is, the powers of $k$ are the same, each propagator has a momentum integral, each vertex has a delta function, and each vertex involves one $\phi$ line and two fermion lines~\cite[p.~316]{Peskin}.  So we can adapt P\&S~(10.4) for the superficial degree of divergence:
	\eq{
		D = 4 - \Nphi - \frac{3}{2} \Nf,
	}
	where $\Nphi$ is the number of external $\phi$ lines and $\Nf$ is the number of external fermion lines.
	
	This means the superficially divergent amplitudes are a subset of those appearing in Fig.~10.2 of P\&S, with the photon lines replaced by pseudoscalar lines: \\[-4ex]
	\al{
		\text{(a)} &\: \centergraphics{diag/amp_a} \quad D = 4 &
		\text{(b)} &\: \centergraphics{diag/amp_b} \quad D = 3 &
		\text{(c)} &\: \centergraphics{diag/amp_c} \quad D = 2 \\
		\text{(d)} &\: \centergraphics{diag/amp_d} \quad D = 1 &
		\text{(e)} &\: \centergraphics{diag/amp_e} \quad D = 0 &
		\text{(f)} &\: \centergraphics{diag/amp_f} \quad D = 1 \\
		& &
		\text{(g)} &\: \centergraphics{diag/amp_g} \quad D = 0 &
	}
	We ignore (a) since it is irrelevant to scattering processes~\cite[pp.~317--318]{Peskin}.  Amplitudes~(b) and (d) vanish because the theory is invariant under the parity transformation, which means all amplitudes with zero external fermion legs and an odd number of external $\phi$ legs vanish~\cite[pp.~318, 323--324]{Peskin}.  So the superficially divergent amplitudes are \\[-3ex]
	\ans{\al{
		\text{(c)} &\: \centergraphics{diag/blue_amp_c} \quad D = 2 &
		\text{(e)} &\: \centergraphics{diag/blue_amp_e} \quad D = 0 &
		\text{(f)} &\: \centergraphics{diag/blue_amp_f} \quad D = 1 \\
		& &
		\text{(g)} &\: \centergraphics{diag/blue_amp_g} \quad D = 0 &
	}}%
	\ans{Note that amplitude~(e) is a $4\phi$ amplitude.}  Since it is superficially divergent, according to the problem statement  we must introduce the scalar self-interaction given by Eq.~\refeq{given1a}.  We subtract this term as in the $\phi^4$ theory~\cite[p.~324]{Peskin}.  The Feynman rule for this vertex is~\cite[p.~325]{Peskin}
	\eq{
		\centergraphics{diag/scalar_vertex} = -i \lamo.
	}
	With the addition of this new term, our Lagrangian in Eq.~\refeq{newlagr} becomes
	\eqn{newlagr2}{
		\cL = \frac{1}{2} (\ptsm \phi)^2 - \frac{1}{2} \mo^2 \phi^2 + \psib (i \ptsl - \Mo) \psi - i \go \psib \gamt \psi \phi - \frac{\lamo}{4!} \phi^4,
	}
	where $\lamo$ is the bare coupling constant for the scalar self-interaction.  To work out the renormalized theory, we rescale the field as in P\&S~(10.15):
	\eq{
		\phi = \Zq^{1/2} \phir.
	}
	The rescaling for the fermion is~\cite[p.~330]{Peskin}
	\eq{
		\psi = \Zw^{1/2} \psir.
	}
	Feeding these into Eq.~\refeq{newlagr2}, we obtain the renormalized Lagrangian~\cite[p.~324]{Peskin}
	\eqn{lagr2}{
		\cL = \frac{1}{2} \Zq (\ptsm \phi)^2 - \frac{1}{2} \Zq \mo^2 \phi^2 + \Zw \psib (i \ptsl - \Mo) \psi - i \Zq^{1/2} \Zw \go \psib \gamt \psi \phi - \frac{\lamo}{4!} \Zq^2 \phi^4.
	}
	Define~\cite[pp.~324, 331]{Peskin}
	\al{
		\delZq &= \Zq - 1, &
		\delZw &= \Zw - 1, &
		\delm &= \mo^2 \Zq - m^2, \\
		\delM &= \Mo \Zw - M, &
		\delg &= (\go / g) \Zq^{1/2} \Zw - 1, &
		\dellam &= \lamo \Zq^2 - \lam
	}
	Then Eq.~\refeq{lagr2} becomes
	\al{
		\cL &= \frac{1}{2} (1 + \delZq) (\ptsm \phi)^2 - \frac{1}{2} (m^2 + \delm) \phi^2 + \psib [ i (\delZw + 1) \ptsl - (M + \delM) ] \psi - i g (1 + \delg) \psib \gamt \psi \phi + \frac{\lam + \dellam}{4!} \phi^4 \\[2ex]
		&= \frac{1}{2} (\ptsm \phi)^2 - \frac{1}{2} m^2 \phi^2 + \psib (i \ptsl - M) \psi - i g \psib \gamt \psi \phi - \frac{\lam}{4!} \phi^4 \\
		&\hspace{5em} \phantom{=\ } + \frac{1}{2} \delZq (\ptsm \phi)^2 - \frac{1}{2} \delm \phi^2 + \psib (i \delZw \ptsl - \delM) \psi - i g \delg \psib \gamt \psi \phi - \frac{\dellam}{4!} \phi^4.
	}
	Here the first first five terms look like Eq.~\refeq{newlagr2}, but written in terms of the physical masses and couplings.  The last five terms are the counterterms~\cite[p.~325]{Peskin}.
	
	The Feynman rules for the renormalized theory are \\[-5ex]
	\ans{\al{
		\centergraphics{diag/blue_scalar_prop} &= \frac{i}{q^2 - m^2 + i \eps} &
		\centergraphics{diag/ren_scalar_prop} &= i (p^2 \delZq - \delm) \\
		\centergraphics{diag/blue_fermion_prop} &= \frac{i (\psl + M)}{p^2 - M^2 + i \eps} &
		\centergraphics{diag/ren_fermion_prop} &= i (\psl \delZw - \delM) \\
		\centergraphics{diag/blue_scalar_fermion_vertex} &= g \gamt &
		\centergraphics{diag/ren_scalar_fermion_vertex} &= g \delg \gamt \\
		\centergraphics{diag/blue_scalar_vertex} &= -i \lam &
		\centergraphics{diag/ren_scalar_vertex} &= -i \dellam
	}}%
	
	\hl{why we don't need any more interactions}
}



\prob{
	Compute the divergent part (the pole as $d \to 4$) of each counterterm, to the one-loop order of perturbation theory, implementing a sufficient set of renormalization conditions.  You need not worry about finite parts of the counterterms.  Since the divergent parts must have a fixed dependence on the external momenta, you can simplify this calculation by choosing the momenta in the simplest possible form.
}

\sol{
	To compute the divergent part of the fermion propagator counterterm to one-loop order, we include the fermion self-energy: \hl{(draw the diagram)}
	
	The fermion-self energy here looks similar to that in QED, so we may adapt P\&S~(7.16) for that term.  Using our Feynman rules from \ref{1a}, we have
	\aln{
		-i \Sigwp &= i (\psl \delZw - \delM) + g^2 \int \dddkf \gamt \frac{i (\ksl + M)}{p^2 - M^2 + i \eps} \gamt \frac{i}{(p - k)^2 - m^2 + i \eps} \notag \\
		&= i (\psl \delZw - \delM) + g^2 \int \dddkf \frac{\ksl - M}{(p^2 - M^2 + i \eps) [ (p - k)^2 - m^2 + i \eps ]} \label{thing1b2},
	}
	where we have used P\&S~(3.70), $(\gamt)^2 = 1$, and (3.71), $\{ \gamt, \gamm \} = 0$, which implies $\gamt \gamm \gamt = -\gamm$.  Following the procedure on pp.~217--218, we introduce the Feynman parameter $x$ to combine the denominators:
	\eqn{FP}{
		\frac{1}{k^2 - \mo^2 + i \eps} \frac{1}{(p - k)^2 - \mu^2 + i \eps} = \intoq \ddx \frac{1}{[ k^2 - 2 x k \cdot p + x p^2 - x \mu^2 - (1 - x) \mo^2 + i \eps ]^2}.
	}
	Let $\ell = k - x p$ and $\Del = -x(1 - x) p^2 + x m^2 + (1 - x) M^2$.  Then Eq.~\refeq{thing1b2} can be written
	\eqn{thing1b2b}{
		-i \Sigwp = i (\psl \delZw - \delM) + g^2 \intoq \ddx \int \dddlf \frac{(x \psl - M)}{[ \ell^2 - \Del + i \eps ]^2}.
	}
	To evaluate the integral, we can write it in terms of the Euclidean 4-momentum defined by~\cite[p.~193]{Peskin}
	\aln{ \label{ellE}
		\ello &\equiv i \ellEo, &
		\vell &= \vellE.
	}
	Then we can write
	\eq{
		\int \dddlf \frac{1}{(\ell^2 - \Del)^2} = \frac{i}{(-1)^2} \frac{1}{(2\pi)^d} \int \dddlE \frac{1}{(\ellE^2 + \Del)^2}
		= i \int \dddlEf \frac{1}{(\ellE^2 + \Del)^2}.
	}
	Then we can apply (7.84), which takes the limit as $d \to 4$:
	\eq{
		\int \dddlEf \frac{1}{(\ellE^2 + \Del)^2} \to \frac{1}{(4\pi)^2} \paren{ \frac{2}{\eps} - \gam + \ln(\frac{4\pi}{\Del}) }
		\approx \frac{1}{8 \pi^2 \eps},
	}
	where $\eps = 4 - d$~\cite[p.~250]{Peskin}, and we have omitted the finite parts.  Making these substitutions into Eq.~\refeq{Sigw2}, we find
	\al{
		-i \Sigwp &= i (\psl \delZw - \delM) + \frac{i g^2}{8 \pi^2 \eps} \intoq \ddx (x \psl - M) \\
		&= i (\psl \delZw - \delM) + \frac{i g^2}{8 \pi^2 \eps} \brac{ \frac{x^2}{2} \psl - M x }_0^1 \\
		&= i (\psl \delZw - \delM) + \frac{i g^2}{8 \pi^2 \eps} \paren{ \frac{\psl}{2} - M } \\
		&= i \psl \paren{ \delZw + \frac{g^2}{16 \pi^2 \eps} } - i \paren{ \delM + \frac{g^2}{8 \pi^2 \eps} M }.
	}
	This implies
	\ans{\al{
		\delZq &= -\frac{g^2}{16 \pi^2 \eps}, &
		\delM &= -\frac{g^2}{8 \pi^2 \eps} M
	}}%
	are the conditions to eliminate the divergence.
	
	For the scalar-fermion vertex, we can adapt some of our work from problem~2 of Homework~1.  We adapt Peskin \& Schroeder (6.38) using the pseudoscalar field Feynman rules to write~\cite[p.~123]{Peskin}
	\aln{
		\ubpp \del\Gamm(p, p') \up &= \ubpp g \delg \gamt \up + g^3 \int \dddkf \ubpp \frac{\gamt (\ksl' + M) \gamt (\ksl + M) \gamt}{[ (k - p)^2 - m^2 + i \eps ] ({k'}^2 - M^2 + i \eps) (k^2 - M^2 + i \eps)} \up \notag \\
		&= \ubpp g \delg \gamt \up + g^3 \gamt \int \dddkf \ubpp \frac{(\ksl' + M) (\ksl - M)}{[ (k - p)^2 - m^2 + i \eps ] ({k'}^2 - M^2 + i \eps) (k^2 - M^2 + i \eps)} \up, \label{thing1bc}
	}
	where we have once more used $(\gamt)^2 = 1$.  We use Peskin \& Schroeder~(6.41) to write 
	\eqn{denom}{
		\frac{1}{[ (k - p)^2 - m^2 + i \eps ] ({k'}^2 - M^2 + i \eps) (k^2 - M^2 + i \eps)} = \intoq \ddx \ddy \ddz \del(x + y + z - 1) \frac{2}{D^3},
	}
	where~\cite[pp.~190--191]{Peskin}
	\eq{
		D = k^2 + 2 k (q y - p z) + z (p^2 - m^2) - (1 - z) M^2 + i \eps
		= k^2 - 2 k p z + z (p^2 - m^2) - (1 - z) M^2 + i \eps
		\equiv \ell^2 - \Del + i \eps.
	}
	Here we have used $x + y + z = 1$ and set $q = 0$ (so $k' = k$) as in problem~2 of Homework~1.  We have defined $\ell \equiv k - z p$~\cite[p.~191]{Peskin}, and
	\eq{
		\Del \equiv (1 - z)^2 M^2 + z m^2.
	}
	For the numerator of Eq.~\refeq{thing1bc}, we use $\ell \equiv k - z p$~\cite[p.~191]{Peskin}, and define
	\eqn{N1}{
		N \equiv \ubpp \gamt (\ell + z p + M) (\ell + z p - M) \up
	}
	
	\hl{finish later}
}


\makebib

\end{document}
