\newcommand{\kpsi}{\ket{\psi}}
\newcommand{\kup}{\ket{\uparrow}}
\newcommand{\kdn}{\ket{\downarrow}}
\newcommand{\cq}{c_1}
\newcommand{\cw}{c_2}
\newcommand{\cqs}{c_1^*}
\newcommand{\cws}{c_2^*}
\newcommand{\kbpsi}{\ketbra{\psi}}

\section{Problem 3}
\begin{statement}
	Consider a spin $1/2$ state $\kpsi = \cq \kup + \cw \kdn$, where $\kup$ and $\kdn$ are the $\Sz$ eigenstates with eigenvalues $+\hbar/2$ and $-\hbar/2$, respectively.
\end{statement}

\begin{problem} \label{3.1}
	Consider the operator $\rho = \kbpsi$.  Write down the matrix elements of $\rho$ in the basis $\{ \kup, \kdn \}$.
\end{problem}

\begin{solution}
	From the definition of $\kpsi$,
	\begin{align*}
		\braket{\up}{\psi} &= \cq, &
		\braket{\psi}{\up} &= \cqs, &
		\braket{\dn}{\psi} &= \cw, &
		\braket{\psi}{\dn} &= \cws.
	\end{align*}
	Using these,
	\begin{align*}
		\mel{\up}{\rho}{\up} &= \braket{\up}{\psi} \braket{\psi}{\up} = \cq \cqs = |\cq|^2, &
		\mel{\up}{\rho}{\dn} &= \braket{\up}{\psi} \braket{\psi}{\dn} = \cq \cws, \\
		\mel{\dn}{\rho}{\up} &= \braket{\dn}{\psi} \braket{\psi}{\up} = \cqs \cw, &
		\mel{\dn}{\rho}{\dn} &= \braket{\dn}{\psi} \braket{\psi}{\dn} = \cw \cws = |\cw|^2.
	\end{align*}
	In matrix form,
	\beqn \label{matrho}
		\rho = \mqty[ |\cq|^2 & \cq \cws \\ \cqs \cw & |\cw|^2 ].
	\eeqn
\vfix
\end{solution}

\newcommand{\soo}{s_0}
\newcommand{\sq}{s_1}
\newcommand{\sw}{s_2}
\newcommand{\se}{s_3}
\newcommand{\vs}{\vec{s}}

\newcommand{\Recq}{\Re(\cq)}
\newcommand{\Imcq}{\Im(\cq)}
\newcommand{\Recw}{\Re(\cw)}
\newcommand{\Imcw}{\Im(\cw)}

\newcommand{\sds}{\vs \cdot \vsig}

\begin{problem}
	In the $\Sz$ eigenbasis, express $\rho$ by using the Pauli matrices.  That is, write $\rho$ as
	\beqn \label{exprho}
		\rho = \frac{\soo}{2} I + \frac{1}{2} \sds,
	\eeqn
	and express $\soo, \sq, \sw, \se$ in terms of $\cq$ and $\cw$.
\end{problem}

\begin{solution}
	Expanding \refeq{exprho} using the Pauli matrices given by \refeq{pauli},
	\beq
		\rho = \frac{1}{2} \mqty[ \soo & 0 \\ 0 & \soo ] + \frac{1}{2} \mqty[ 0 & \sq \\ \sq & 0 ] + \frac{i}{2} \mqty[ 0 & -\sw \\ \sw & 0 ] + \frac{1}{2} \mqty[ \se & 0 \\ 0 & -\se ]
		= \frac{1}{2} \mqty[ \soo + \se & \sq - i \sw \\ \sq + i \sw & \soo - \se ].
	\eeq
	Matching up the matrix elements with those in \refeq{matrho}, we have a system of four equations:
	\begin{align*}
		\frac{\soo + \se}{2} &= |\cq|^2 &
		\frac{\sq - i \sw}{2} &= \cq \cws &
		\frac{\sq + i \sw}{2} &= \cqs \cw &
		\frac{\soo - \se}{2} &= |\cw|^2.
	\end{align*}
	Solving these for $\soo, \sq, \sw, \se$,
	\begin{align}
		\soo &= \frac{\soo + \se}{2} + \frac{\soo - \se}{2}
		= |\cq|^2 + |\cw|^2, &
		\sq &= \frac{\sq - i \sw}{2} + \frac{\sq + i \sw}{2}
		= \cq \cws + \cqs \cw, \label{scomp} \\
		\sw &= i \left( \frac{\sq - i \sw}{2} - \frac{\sq + i \sw}{2} \right)
		= i (\cq \cws - \cqs \cw), &
		\se &= \frac{\soo + \se}{2} - \frac{\soo - \se}{2}
		= |\cq|^2 - |\cw|^2. \label{scomp2}
	\end{align}
	Note that $\soo$ is the norm of $\kpsi$, so $\soo = 1$ assuming $\kpsi$ is normalized.  Then \refeq{exprho} can be written
	\begin{align*}
		\rho &= \frac{|\cq|^2 + |\cw|^2}{2} I + \frac{\cq \cws + \cqs \cw}{2} \sigx + i \frac{\cq \cws - \cqs \cw}{2} \sigy + \frac{|\cq|^2 - |\cw|^2}{2} \sigz \\
		&= \frac{1}{2} I + \frac{\cq \cws + \cqs \cw}{2} \sigx + i \frac{\cq \cws - \cqs \cw}{2} \sigy + \frac{|\cq|^2 - |\cw|^2}{2} \sigz.
	\end{align*}
\vfix
\end{solution}

\begin{problem}
	Compute $\rho^2$ and $\vs^2$.
\end{problem}

\begin{solution}
	Using the representation of $\rho$ in \refeq{exprho},
	\beq
		\rho^2 = \frac{\soo^2}{4} I^2 + \frac{\soo}{4} I (\sds) + \frac{\soo}{4} (\sds) I + \frac{1}{4} (\sds)^2
		= \frac{1}{4} (\soo^2 + |\vs|^2) I + \frac{\soo}{2} \sds
		= \frac{1}{4} (1 + |\vs|^2) I + \frac{1}{2} \sds,
	\eeq
	where $\vs = (\sq, \sw, \se)$, and in the final equality we have assumed $\kpsi$ is normalized.  Using \refeq{scomp} and \refeq{scomp2},
	\begin{align*}
		\vs^2 &= \vs \cdot \vs = \sq^2 + \sw^2 + \se^2
		= \left( \cq \cws + \cqs \cw \right)^2 - \left( \cq \cws - \cqs \cw \right)^2 + \left( |\cq|^2 - |\cw|^2 \right)^2 \\
		&= \cq^2 {\cws}^2 + 2 |\cq|^2 |\cw|^2 + {\cqs}^2 \cw^2 - \cq^2 {\cws}^2 + 2 |\cq|^2 |\cw|^2 - {\cqs}^2 \cw^2 + |\cq|^4 - 2 |\cq|^2 |\cw|^2 + |\cw|^4 \\
		&= |\cq|^4 + 2 |\cq|^2 |\cw|^2 + |\cw|^4
		= \left( |\cq|^2 + |\cw|^2 \right)^2 \\
		&= \soo^2 = 1.
	\end{align*}
	We can use this result to simplify the expression for $\rho^2$:
	\beq
		\rho^2 = \frac{1}{2} \soo^2 I + \frac{\soo}{2} \sds = \rho.
	\eeq
\vfix
\end{solution}

\newcommand{\bpsi}{\bra{\psi}}
\newcommand{\rhot}{\rho(t)}

\begin{problem}
	Using the {\Schrodinger} equation
	\beqn \label{schro}
		i \hbar \dv{}{t} \kpsi = H \kpsi,
	\eeqn
	derive the equation of motion obeyed by $\rho$.
\end{problem}

\begin{solution}
	The adjoint of \refeq{schro} is
	\beq
		-i \hbar \pdv{}{t} \bpsi = \bpsi H
		\iff
		i \hbar \pdv{}{t} \bpsi = -\bpsi H.
	\eeq
	Then
	\begin{align*}
		i \hbar \dv{\rho}{t} = i \hbar \dv{}{t} \kbpsi
		= H \kbpsi - \kbpsi H
		= H \rho - \rho H
		= [H, \rho],
	\end{align*}
	so the equation of motion is
	\beq
		\dv{\rho}{t} = \frac{i}{\hbar} [\rho, H].
	\eeq
\vfix
\end{solution}

\newcommand{\vOme}{\boldsymbol{\Omega}}
\newcommand{\psiu}{\psi_\up}
\newcommand{\psid}{\psi_\dn}
\newcommand{\psiut}{\psiu(t)}
\newcommand{\psidt}{\psid(t)}
\newcommand{\kpsit}{\ket{\psit}}
\newcommand{\Ods}{\vOme \cdot \vsig}
\newcommand{\Omx}{\Omega_x}
\newcommand{\Omy}{\Omega_y}
\newcommand{\Omz}{\Omega_z}

\newcommand{\vaa}{\vec{a}}
\newcommand{\vbb}{\vec{b}}
\newcommand{\costt}{\cos{\frac{t}{2}}}
\newcommand{\sintt}{\sin{\frac{t}{2}}}

\begin{problem}
	When the Hamiltonian is given by
	\beqn \label{ham3}
		H = \frac{\hbar}{2} \Ods,
	\eeqn
	write down the equation of motion obeyed by $(\psiut, \psidt)$, where $\psiut, \psidt$ are the (complex) expansion coefficients of the state ket
	\beq
		\kpsit = \psiut \kup + \psidt \kdn.
	\eeq
\vfix
\end{problem}

\begin{solution}
	Using \refeq{schro},
	\beq
		i \hbar \dv{}{t} \kpsit = \frac{\hbar}{2} \Ods \kpsit
		\iff
		i \hbar \dv{}{t} \left( \psiut \kup + \psidt \kdn \right) = \frac{\hbar}{2} \Ods \left( \psiut \kup + \psidt \kdn \right),
	\eeq
	which can be separated into two equations:
	\begin{align}
		\dv{}{t} \psiut \kup &= -\frac{i}{2} \psiut \, \Ods \kup, &
		\dv{}{t} \psidt \kdn &= -\frac{i}{2} \psidt \, \Ods \kdn.
	\end{align}
	Generalizing the results of \ref{2.1}, let $\vOme = \Omega \, \vn$ where $\vn$ is a unit vector.  Using \refeq{ndsmat},
	\begin{align*}
		\Ods \kup &= \Omega \mqty[ \nz \\ \nx + i \ny ] = \Omz \kup + (\Omx + i \Omy) \kdn, &
		\Ods \kdn &= \Omega \mqty[ \nx - i \ny \\ -\nz ] = (\Omx - i \Omy) \kup - \Omz \kdn,
	\end{align*}
	where $\vOme = (\Omx, \Omy, \Omz)$.  Then, explicitly, we have the equations of motion
	\begin{align}
		\dv{}{t} \psiut \kup &= -\frac{i}{2} \psiut \left[ \Omz \kup + (\Omx + i \Omy) \kdn \right], &
		\dv{}{t} \psidt \kdn &= -\frac{i}{2} \psidt \left[ (\Omx - i \Omy) \kup - \Omz \kdn \right].
	\end{align}
\vfix
\end{solution}

\newcommand{\sigi}{\sig_i}
\newcommand{\sigj}{\sig_j}
\newcommand{\sigk}{\sig_k}
\newcommand{\lct}{\varepsilon_{ijk}}
\newcommand{\Sq}{S_1}
\newcommand{\Sw}{S_2}
\newcommand{\Se}{S_3}
\newcommand{\Si}{S_i}
\newcommand{\Omq}{\Omega_1}
\newcommand{\Omw}{\Omega_2}
\newcommand{\Ome}{\Omega_3}
\newcommand{\Omj}{\Omega_j}

\newcommand{\Sx}{S_x}

\begin{problem}
	When the Hamiltonian is given by \refeq{ham3}, write down the (Heisenberg) equation of motion obeyed by the spin operators $\vS$.
\end{problem}

\begin{solution}
	From (3.2.35) in Sakurai,
	\beq
		[\sigi, \sigj] = 2 i \lct \sigk
	\eeq
	Let $\vS = (\Sq, \Sw, \Se)$ and $\vOme = (\Omq, \Omw, \Ome)$.  Then the Heisenberg equation of motion is
	\beq
		\dv{\Si}{t} = -\frac{i}{\hbar} [\Si, H] = -\frac{i \hbar}{4} [\sigi, \Ods] = -\frac{i \hbar}{4} \sum_{j = 1}^3 \Omj [\sigi, \sigj] = \frac{\hbar}{2} \sum_{j = 1}^3 \Omj \lct \sigk.
	\eeq
	Explicitly, the equations of motion are
	\begin{align*}
		\dv{\Sx}{t} &= \frac{\hbar}{2} (\Omy \sigz - \Omz \sigy), &
		\dv{\Sy}{t} &= \frac{\hbar}{2} (\Omz \sigx - \Omx \sigz), &
		\dv{\Sz}{t} &= \frac{\hbar}{2} (\Omx \sigy - \Omy \sigx).
	\end{align*}
\end{solution}