\documentclass[11pt]{article}
\usepackage{homework}

\classname{443}
\homeworknum{2}



\begin{document}

\input{definitions}
\input{probdefs}


\input{Problem1}






\state{(Peskin \& Schroeder 3.1) \hspace{1em} Lorentz group}{
	Recall from Eq.~(3.17) the Lorentz commutation relations,
	\eq{
		[\Jmn, \Jrs] = i (\gnr \Jms - \gmr \Jns - \gns \Jmr + \gms \Jnr).
	}
}

\prob{}{
	Define the generators of rotations and boosts as
	\al{
		\Li &= \frac{1}{2} \epsijk \Jjk, &
		\Ki &= \Joi,
	}
	where $i, j, k = 1, 2, 3$.  An infinitesimal Lorentz transformation can then be written
	\eq{
		\Phi \to (1 - i \vtht \vdot \vL - i \vbet \vdot \vK) \Phi.
	}
	Write the commutation relations of these vector operators explicitly.  (For example, $[\Li, \Lj] = i \epsijk \Lk$.)  Show that the combinations
	\al{
		\vJp &= \frac{1}{2} (\vL + i \vK), &
		\vJm &= \frac{1}{2} (\vL - i \vK)
	}
	commute with one another and separately satisfy the commutation relations of angular momentum.
}

\sol{
	Firstly, using the Eq.~(3.18)
	\al{
		[\Li, \Lj] &= \brac{ \frac{1}{2} \epsimn \Jmn, \frac{1}{2} \epsjrs \Jrs }
		= \frac{1}{4} \epsimn \epsjrs [\Jmn, \Jrs]
		= \frac{i}{4} \epsimn \epsjrs (\gnr \Jms - \gmr \Jns - \gns \Jmr + \gms \Jnr) \\
		&= \frac{i}{4} (\epsimn \epsjrs \gnr \Jms - \epsimn \epsjrs \gmr \Jns - \epsimn \epsjrs \gns \Jmr + \epsimn \epsjrs \gms \Jnr) \\
		&= \frac{i}{4} (\epsimn \epsjrs \gnr \Jms - \epsinm \epsjrs \gnr \Jms - \epsimn \epsjsr \gnr \Jms + \epsinm \epsjsr \gnr \Jms) \\
		&= \frac{i}{4} (\epsimn \epsjrs \gnr \Jms + \epsimn \epsjrs \gnr \Jms + \epsimn \epsjrs \gnr \Jms + \epsimn \epsjrs \gnr \Jms) \\
		&= i \epsimn \epsjrs \gnr \Jms,
	}
	where we have simply relabeled indices.  Then, using $\gsab = \delsab$~\cite{Metric} and $\epsijk \epspqk = \delip \deljq - \deliq \deljp$~\cite{LeviCivita},
	\al{
		[\Li, \Lj] &= i \epsimsn \epsjrs \delsnr \Jms
		= i \epsimsn \epsjns \Jms
		= i \epsimn \epsjsn \Jms
		= i (\delij \delms - \delis \delmj) \Jms
		= i (\delij \Jmm - \delis \Jjs)
		= -i \Jji \\
		&= i \Jij,
	}
	where we have used the antisymmetry of $\Jij$.  From $\Li = \frac{1}{2} \epsijk \Jjk$, we can write
	\eq{
		\epsirs \Li = \frac{1}{2} \epsijk \epsirs \Jjk
		= \frac{1}{2} (\deljr \delks - \deljs \delkr) \Jjk
		= \frac{1}{2} (\deljr \Jjs - \deljs \Jjr)
		=  \frac{1}{2} (\Jrs - \Jsr)
		= \Jrs.
	}
	Then we see that
	\eq{
		\ans{ [\Li, \Lj] = i \epsijk \Lk. }
	}
	
	Secondly,
	\eq{
		[\Ki, \Kj] = [\Joi, \Joj]
		= i (\gio \Joj - \goo \Jij - \gij \Joo + \goj \Jio)
		= -i \Jij
		= \ans{ -i \epsijk \Lk.=, }
	}
	and thirdly,
	\al{
		[\Ki, \Lj] &= \brac{ \Joi, \frac{1}{2} \epsjrs \Jrs }
		= \frac{1}{2} \epsjrs [\Joi, \Jrs]
		= \frac{i}{2} \epsjrs (\gir \Jos - \gor \Jis - \gis \Jor + \gos \Jir) \\
		&= \frac{i}{2} (\epsjrs \gir \Jos - \epsjrs \gis \Jor)
		= \frac{i}{2} (\epsjrs \gir \Jos - \epsjsr \gir \Jos)
		= i \epsjrs \gir \Jos
		= i \epsjsrs \delsri \Jos
		= -i \epsijs \Jos \\
		&= \ans{ -i \epsijk \Kk. }
	}
}



\prob{}

}




%\state{Peskin \& Schroeder 3.4}{
%
%}
%
%
%
%
%\state{Peskin \& Schroeder 3.7}{
%
%}

\clearpage
\makebib

\end{document}
