\state{(Peskin \& Schroeder 7.3)}{
	Consider a theory of elementary fermions that couple both to QED and to a Yukawa field $\phi$:
	\eqn{diag}{
		\Hint = \int \ddcx \frac{\lam}{\sqrt{2}} \phi \psib \psi + \int \ddcx e \Asm \psib \gamm \psi.
	}
}

\prob{ \label{2a}
	Verify that the contribution to $\Zq$ from the vertex diagram with a virtual $\phi$ equals the contribution to $\Zw$ from the diagram with a virtual $\phi$.  Use dimensional regularization.  Is the Ward identity generally true in this theory?
}

\sol{
	We begin by finding $\del\Zq$.  We are interested in the diagram 
	\eqn{diag}{
		\centergraphics{diag/loop}
	}
	We considered a similar diagram in Homework~6 of Physics~443, and we build on that work here.  We adapted Peskin \& Schroeder (6.38) using the scalar field Feynman rules to write~\cite[p.~123]{Peskin}
	\aln{
		\ubpp \del\Gamm(p, p') \up &= \int \dddkf \frac{i}{(k - p)^2 - \mphi^2 + i \eps} \ubpp \paren{ -i \frac{\lam}{\sqrt{2}} } \frac{i (\ksl' + \me)}{{k'}^2 - \me^2 + i \eps} \gamm \frac{i (\ksl + \me)}{k^2 - \me^2 + i \eps} \paren{ -i \frac{\lam}{\sqrt{2}} } \up \notag \\
		&= \frac{i \lam^2}{2} \int \dddkf \ubpp \frac{(\ksl' + \me) \gamm (\ksl + \me)}{[ (k - p)^2 - \mphi^2 + i \eps ] ({k'}^2 - \me^2 + i \eps) (k^2 - \me^2 + i \eps)} \up. \label{thing1a}
	}
	We use Peskin \& Schroeder~(6.41) to write 
	\eqn{denom}{
		\frac{1}{[ (k - p)^2 - \mphi^2 + i \eps ] ({k'}^2 - \me^2 + i \eps) (k^2 - \me^2 + i \eps)} = \intoq \ddx \ddy \ddz \del(x + y + z - 1) \frac{2}{D^3},
	}
	where~\cite[pp.~190--191]{Peskin}
	\eqn{D}{
		D = k^2 + 2 k (q y - p z) + z (p^2 - \mphi^2) - (1 - z) \me^2 + i \eps
		\equiv \ell^2 - \Del + i \eps,
	}
	where we use $x + y + z = 1$ and $k' = k + q$, and we have defined $\ell \equiv k + y q - z p$~\cite[p.~191]{Peskin}, and
	\eq{
		\Del \equiv -x y q^2 + (1 - z)^2 \me^2 + z \mphi^2.
	}
	For the numerator of Eq.~\refeq{thing1a}, we use $k' = k + q$ and $\ell \equiv k + y q - z p$~\cite[p.~191]{Peskin}, and define
	\eqn{N1}{
		N \equiv \ubpp [ \lsl + (1 - y) \qsl + z \psl + \me ] \gamm (\lsl - y \qsl + z \psl + \me) \up
	}
	Again discarding terms linear in $\ell$, Eq.~\refeq{N1} simplifies to
	\aln{
		N &= \ubpp [ \lsl \gamm \lsl - y (1 - y) \qsl \gamm \qsl + z (1 - y) \qsl \gamm \psl + \me (1 - y) \qsl \gamm - y z \psl \gamm \qsl + z^2 \psl \gamm \psl + \me z \psl \gamm - \me y \gamm \qsl \notag \\
		&\hspace{5em} \phantom{=\ } + \me z \gamm \psl + \me^2 \gamm ] \up. \label{N2}
	}
	Using Eqs.~\refeq{id1}--\refeq{id4}, the terms above reduce to
	\al{
		\lsl \gamm \lsl &= (2 \ellm - \gamm \lsl) \lsl
		= 2 \ellm \elln \gamsn - \gamm \lsl \lsl
		\to \frac{2}{d} \ell^2 \gmn \gamsn - \gamm \ell^2
		\to \frac{2 - d}{d} \ell^2 \gamm - 2 \me^2 \gamm
		= 0,
		\\
		\qsl \gamm \qsl &\to  0,
		\\
		\qsl &\to 0,
		\\
		\qsl \gamm &\to 0,
		\\
		\psl \gamm \qsl &\to 0, \\
		\psl \gamm \psl &\to \me \psl \gamm
		= \me (2 \pmu - \gamm \psl)
		\to 2 \me \pmu - \me^2 \gamm
		\to 2 \me^2 \gamm - \me^2 \gamm
		= \me^2 \gamm,
		\\
		\psl \gamm &= 2 \pmu - \gamm \psl
		= 2 \pmu - \gamm \me
		\to 2 \me \gamm - \gamm \me
		= \me \gamm,
		\\
		\gamm \qsl &\to 0,
		\\
		\gamm \psl &\to \me \gamm.
	}
	Feeding these back into Eq.~\refeq{N2}, we obtain
	\al{
		N \to \ubpp \brac{ \frac{2 - d}{d} \ell^2 + z^2 \me^2 + \me^2 z + \me^2 z + \me^2 } \gamm \up
		= \ubpp \brac{ \frac{2 - d}{d} \ell^2 + (1 + z)^2 \me^2 } \gamm \up.
	}
	Then, letting $\Delo = (1 - z)^2 \me^2 + z \mphi^2$,
	\aln{
		\del\Zq &= -\del\Fq \notag \\
		&= -i \lam^2 \int \dddlf \intoq \ddx \ddy \ddz \del(x + y + z - 1) \frac{(2 - d) \ell^2 / d + (1 + z)^2 \me^2}{(\ell^2 - \Delo)^3}  \notag \\
		&= -i \lam^2 \int \dddlf \intoq \ddz (1 - z) \frac{(2 - d) \ell^2 / d + (1 + z)^2 \me^2}{(\ell^2 - \Delo)^3}.  \label{thing3a}
	}
	Applying Eqs.~\refeq{int1} and \refeq{int2}, Eq.~\refeq{thing3a} becomes
	\aln{
		\del\Zq &= -i \lam^2 \intoq \ddz (1 - z) \brac{ \frac{2 - d}{d} \frac{i}{(4\pi)^{2 - \eps / 2}} \frac{d}{2} \frac{\Gam(\eps / 2)}{\Gam(3)} \paren{ \frac{1}{\Delo} }^{\eps / 2} - (1 + z)^2 \me^2 \frac{i}{(4\pi)^{2 - \eps / 2}} \frac{\Gam(1 + \eps / 2)}{\Gam(3)} \paren{ \frac{1}{\Delo} }^{1 + \eps / 2} } \notag \\
		&= \frac{1}{\Gam(3)} \frac{\lam^2}{(4\pi)^{2 - \eps / 2}} \intoq \ddz (1 - z) \brac{ \frac{\eps - 2}{2} \Gam(\eps / 2) \paren{ \frac{1}{\Delo} }^{\eps / 2} - (1 + z)^2 \me^2 \Gam(1 + \eps / 2) \paren{ \frac{1}{\Delo} }^{1 + \eps / 2} } \notag \\
		&= \frac{1}{\Gam(3)} \frac{\lam^2}{(4\pi)^2} \intoq \ddz (1 - z) \brac{ \frac{\eps - 2}{2} \Gam(\eps / 2) \paren{ \frac{4\pi}{\Delo} }^{\eps / 2} - \frac{(1 + z)^2 \me^2}{\Del} \Gam(1 + \eps / 2) \paren{ \frac{4\pi}{\Delo} }^{\eps / 2} } \notag \\
		&\approx -\frac{\lam^2}{32 \pi^2} \intoq \ddz (1 - z) \brac{ \frac{2}{\eps} - \gam + \ln(\frac{4\pi}{\Del}) + \frac{(1 + z)^2 \me^2}{\Del} }, \label{Z1a}
	}
	where we have performed the expansion with Mathematica once more.
	
	Now we must find $\del\Zw$.  We begin with a diagram that looks like that in (7.15) of Peskin \& Schroeder, but with a scalar instead of a photon.  We need to adapt their (7.16) for a scalar field.  Using the Feynman rules for a scalar field~\cite[p.~118]{Peskin}, we write
	\eq{
		-i \Sigwp = \paren{ -\frac{i \lam}{\sqrt{2}} }^2 \int \dddkf \frac{i (\ksl + \me)}{k^2 - \me^2 + i \eps} \frac{i}{(p - k)^2 - \mphi^2 + i \eps}.
	}
	Let $\ell = k - x p$ and $\Del = -x (1 - x) p^2 + x \mphi^2 + (1 - x) \me^2$.  Then from Eq.~\refeq{Sigw2},
	\eqn{Siqwa1}{
		\Sigwp = \frac{i \lam^2}{2} \intoq \ddx \int \dddlf \frac{\lsl + x \psl + \me}{(\ell^2 - \Del + i \eps)^2}
		\to \frac{i \lam^2}{2} \intoq \ddx \int \dddlf \frac{x \psl + \me}{(\ell^2 - \Del + i \eps)^2},
	}
	where we have again dropped terms linear in $\ell$.  Then from (7.85),
	\al{
		\int \dddlf \frac{1}{(\ell^2 - \Del)^2} &= \frac{i}{(-1)^2} \frac{1}{(2\pi)^d} \int \frac{\dddlE}{(\ellE^2 + \Del)^2} \\
		&= i \int \dddlEf \frac{1}{(\ellE^2 + \Del)^2} \\
		&= \frac{i}{(4\pi)^{d / 2}} \frac{\Gam(2 - d/2)}{\Gam(2)} \paren{ \frac{1}{\Del} }^{2 - d/2} \\
		&= \frac{i}{(4\pi)^{2 - \eps / 2}} \frac{\Gam(\eps / 2)}{\Gam(2)} \paren{ \frac{1}{\Del} }^{\eps / 2}.
	}
	Feeding this into Eq.~\refeq{Sigwa1} and Taylor expanding as before,
	\al{
		\Sigwp &= \frac{i \lam^2}{2} \intoq \ddx (x \psl + \me) \frac{i}{(4\pi)^{2 - \eps / 2}} \frac{\Gam(\eps / 2)}{\Gam(2)} \paren{ \frac{1}{\Del} }^{\eps / 2} \\
		&= -\frac{\lam^2}{32 \pi^2} \intoq \ddx (x \psl + \me) \Gam(\eps / 2) \paren{ \frac{4\pi}{\Del} }^{\eps / 2} \\
		&\approx -\frac{\lam^2}{32 \pi^2} \intoq \ddx (x \psl + \me) \brac{ \frac{2}{\eps} - \gam + \ln(\frac{4\pi}{\Del}) }.
	}
	Note that
	\eq{
		\dv{\Sigwp}{\psl} = -\frac{\lam^2}{32 \pi^2} \intoq \ddx \curly{ \brac{ \frac{2}{\eps} - \gam + \ln(\frac{4\pi}{\Del}) } \dv{\psl}(x \psl + \me) + (x \psl + \me) \dv{\Del}\brac{ \frac{2}{\eps} - \gam + \ln(\frac{4\pi}{\Del}) } \dv{\Del}{\psl} },
	}
	where
	\al{
		\dv{\psl}(x \psl + \me) &= x, &
		\dv{\Del}\brac{ \frac{2}{\eps} - \gam + \ln(\frac{4\pi}{\Del}) } &= -\frac{1}{\Del}, &
		\dv{\Del}{\psl} &= -2x (1 - x) \psl.
	}
	Then
	\eq{
		\dv{\Sigwp}{\psl} = -\frac{\lam^2}{32 \pi^2} \intoq \ddx \curly{ x \brac{ \frac{2}{\eps} - \gam + \ln(\frac{4\pi}{\Del}) } + (x \psl + \me) \frac{2x (1 - x) \psl}{\Del} },
	}
	so from Eq.~\refeq{Z2},
	\eqn{Zw2a}{
		\del\Zw = -\frac{\lam^2}{32 \pi^2} \intoq \ddx x \brac{ \frac{2}{\eps} - \gam + \ln(\frac{4\pi}{\Delm}) + \frac{2 \me^2 (1 + x) (1 - x)}{\Delm} }.
	}
	Comparing with Eq.~\refeq{Z1a}, we have found
	\ans{\al{
		\del\Zq &= -\frac{\lam^2}{32 \pi^2} \intoq \ddz (1 - z) \brac{ \frac{2}{\eps} - \gam + \ln(\frac{4\pi}{\Del}) + \frac{(1 + z)^2 \me^2}{\Del} }, \\
		\del\Zw &= -\frac{\lam^2}{32 \pi^2} \intoq \ddx x \brac{ \frac{2}{\eps} - \gam + \ln(\frac{4\pi}{\Del}) + \frac{2 \me^2 (1 + x) (1 - x)}{\Del} },
	}}%
	where $\Del = (1 - x)^2 \me^2 + x \mphi^2$.  If the Ward identity is generally true in this theory as we expect, we would have $\del\Zq = \del\Zw$, but it looks like there is a sign error here, at the very least.
}



\prob{
	Now consider the renormalization of the $\phi \psib \psi$ vertex.  Show that the rescaling of this vertex at $q^2 = 0$ is \emph{not} canceled by the correction to $\Zw$.  (It suffices to compute the ultraviolet-divergent parts of the diagrams.)  In this theory, the vertex and field-strength rescaling give additional shifts of the observable coupling constant relative to its bare value.
}

\sol{
	In order to account for both terms of the Hamiltonian, we need to sum the diagrams with scalar propagators and with photon propagators.  Both of the diagrams have scalar external legs.  This means we need to replace Eq.~\refeq{Z1} with a relation that makes sense for a scalar vertex.  We adapt (7.47) as
	\eqn{Gamscalar}{
		\Gam(q = 0) = \Zq^{-1}
		\qimplies
		\del\Gam(q = 0) = -\del\Zq.
	}
	To compute $\del\Zq$, we must sum two vertex diagrams similar to the one on p.~189 of Peskin \& Schroeder.  The first has the external leg replaced with a scalar:
	\aln{
		\ubpp \del\Gamq(p, p') \up &= \int \dddkf \frac{-i \gsnr}{(k - p)^2 + i \eps} \ubpp (-i e \gamn) \frac{i (\ksl' + \me)}{{k'}^2 - \me^2 + i \eps} \frac{i (\ksl + \me)}{k^2 - \me^2 + i \eps} (-i e \gamr) \up \notag \\
		&= -i e^2 \int \dddkf \ubpp \gamn \frac{(\ksl' + \me) (\ksl + \me)}{[ (k - p)^2 + i \eps ] [ {k'}^2 - \me^2 + i \eps ] [ k^2 - \me^2 + i \eps ]} \gamsn \up \label{Gam1}
	}
	We can simplify the calculations at this step (contrary to what we did in \ref{2a}) by setting $q = k' - k = 0$ now.  We introduce Feynman parameters analogously to Eq.~\refeq{denom}.  Let $\ell = k - x p$.  We also introduce the photon mass now, and so define $\Delq = (1 - z)^2 m^2 + z \mu^2$ as in Eq.~\refeq{Delo}.  Then the denominator of the integrand is $\Dq = \ell^2 + \Delq + i \eps$, and the numerator is
	\al{
		\Nq &= \ubpp \gamn (\ksl + \me) (\ksl + \me) \gamsn \up \\
		&= \ubpp \gamn (\lsl + z \psl + \me) (\lsl + z \psl + \me) \gamsn \up \\
		&= \ubpp \gamn (\lsl \lsl + z \lsl \psl + \me \lsl + z^2 \psl \lsl + z \psl \psl + z \me \psl + \me \lsl + z \me \psl + \me^2) \gamsn \up \\
		&\to \ubpp \gamn (\ell^2 + z^2 \me^2 + 2 z \me \psl + \me^2) \gamsn \up \\
%		&= \ubpp (d \ell^2 + d z^2 \me^2 + 2 z \me \gamn \psl \gamsn + d \me^2) \up \\
		&= \ubpp [ d \ell^2 + d z^2 \me^2 + 2 z \me \gamn (2 \psn - \gamsn \psl) + d \me^2 ] \up \\
%		&= \ubpp [ d \ell^2 + d z^2 \me^2 + 2 z \me (2 \psl - d \psl) + d \me^2 ] \up \\
		&= \ubpp [ d \ell^2 + d \me^2 (z^2 + 1) + 2 z \me^2 (2 - d) ] \up,
	}
	where we have dropped terms linear in $\ell$.  Then applying Eqs.~\refeq{Gamscalar} and \refeq{Gam1}, we can write an expression for the contribution to $\del\Zq$, which we call $\del\Zqq$.  We also make use of Eqs.~\refeq{int1} and \refeq{int2}.  We find
	\aln{
		\del \Zqq &= i e^2\intoq \ddz (1 - z) \int \dddlf \frac{d \ell^2 + d \me^2 (z^2 + 1) + 2 z \me^2 (2 - d)}{(\ell^2 + \Delq + i \eps)^3} \notag \\[2ex]
		%
		&= i e^2 \intoq \ddz (1 - z) \left[ \frac{i}{(4\pi)^{2 - \eps / 2}} \frac{(4 - \eps)^2}{2} \frac{\Gam(\eps / 2)}{\Gam(3)} \paren{ \frac{1}{\Delq} }^{\eps / 2} \right. \notag \\
		&\hspace{10em} \phantom{=\ } \left. + \me^2 [ (4 - \eps) (z^2 + 1) + 2 z (\eps - 2) ] \paren{ -\frac{i}{(4\pi)^{2 - \eps / 2}} \frac{\Gam(1 + \eps / 2)}{\Gam(3)} \paren{ \frac{1}{\Delq} }^{1 + \eps / 2} } \notag \right] \notag \\[2ex]
		%
		&= -\frac{e^2}{32 \pi^2} \intoq \ddz (1 - z) \left[ \frac{(4 - \eps)^2}{2} \Gam(\eps / 2) \paren{ \frac{4\pi}{\Delq} }^{\eps / 2} - \frac{\me^2 (z^2 + 1)}{\Delq} (4 - \eps) \Gam(1 + \eps / 2) \paren{ \frac{4\pi}{\Delq} }^{\eps / 2} \right. \notag \\
		&\hspace{25em} \phantom{=\ } \left. - \frac{2 \me^2 z}{\Delq} (\eps - 2) \Gam(1 + \eps / 2) \paren{ \frac{4\pi}{\Delq} }^{\eps / 2} \right] \notag \\[2ex]
		&\approx -\frac{e^2}{32 \pi^2} \intoq \ddz (1 - z) \brac{ \frac{16}{\eps} - 8 - 8 \gam + 8 \ln(\frac{4\pi}{\Delq}) - 4 \frac{\me^2 (z^2 + 1)}{\Delq} + 4 \frac{\me^2 z}{\Delq} } \notag \\[2ex]
		%
		&= -\frac{e^2}{8 \pi^2} \intoq \ddz (1 - z) \brac{ \frac{4}{\eps} - 2 - 2 \gam + 2 \ln(\frac{4\pi}{\Delq}) - \frac{\me^2 (z^2 - z + 1)}{\Delq} }. \label{delZqq}
	}
	
	The second Feynman diagram looks like Eq.~\refeq{diag}, but with a scalar loop instead of a photon loop:
	\aln{
		\ubpp \del\Gamw(p, p') \up &= \int \dddkf \frac{i}{(k - p)^2 - \mphi^2 + i \eps} \ubpp \paren{ -\frac{i \lam}{\sqrt{2}} } \frac{i (\ksl' + \me)}{{k'}^2 - \me^2 + i \eps} \frac{i (\ksl + \me)}{k^2 - \me^2 + i \eps} \paren{ -\frac{i \lam}{\sqrt{2}} } \up \notag \\
		&= \frac{i \lam^2}{2} \int \dddkf \ubpp \frac{(\ksl' + \me) (\ksl + \me)}{[ (k - p)^2 - \mphi^2 + i \eps ] [ {k'}^2 - \me^2 + i \eps ] [ k^2 - \me^2 + i \eps ]} \up \label{Gam2}
	}
	Again setting $q = 0$, we again apply the appropriate analogue to Eq.~\refeq{denom} and let $\Delw = (1 - z)^2 \me^2 + z \mphi^2$.  Then the denominator of the integrand is $\Dw = \ell^2 - \Delw + i \eps$, and the numerator is (again dropping terms linear in $\ell$)
	\al{
		\Nw &= \ubpp (\ksl + \me) (\ksl + \me) \ub \\
		&= \ubpp (\lsl \lsl + z \lsl \psl + \me \lsl + z \psl \lsl + z \psl \psl + z \me \psl + \me \lsl + z \me \psl + \me^2) \ub \\
		&= \ubpp (\ell^2 + 2 z \lsl \me + 2 \me \lsl + z^2 \me^2 + 2 z \me^2 + \me^2) \ub \\
		&\to \ubpp [ \ell^2 + \me^2 (1 + z)^2 ] \ub.
	}
	We call the contribution to $\del\Zq$ from this diagram $\del\Zqw$.  Again using Eqs.~\refeq{int1} and \refeq{int2} yields
	\al{
		\del\Zqw &= -\frac{i \lam^2}{2} \intoq \ddz (1 - z) \int \dddkf \frac{\ell^2 + \me^2 (1 + x)^2}{(\ell^2 - \Delw + i \eps)^3} \\
		&= -\frac{i \lam^2}{2} \intoq \ddz (1 - z) \brac{ \frac{i}{(4\pi)^{2 - \eps / 2}} \frac{4 - \eps}{2} \frac{\Gam(\eps / 2)}{\Gam(3)} \paren{ \frac{1}{\Delw} }^{\eps / 2} - \me^2 (1 + z)^2 \frac{i}{(4\pi)^{2 - \eps / 2}} \frac{\Gam(1 + \eps / 2)}{\Gam(3)} \paren{ \frac{1}{\Delw} }^{1 + \eps / 2} } \\
		&= \frac{\lam^2}{64 \pi^2} \intoq \ddz (1 - z) \brac{ \frac{4 - \eps}{2} \Gam(\eps / 2) \paren{ \frac{4\pi}{\Delw} }^{\eps / 2} - \frac{\me^2 (1 + z)^2}{\Delw} \Gam(1 + \eps / 2) \paren{ \frac{4\pi}{\Delw} }^{1 + \eps / 2} } \\
		&\approx \frac{\lam^2}{64 \pi^2} \intoq \ddz (1 - z) \brac{ \frac{4}{\eps} - 1 - 2 \gam + 2 \ln(\frac{4 \pi}{\Delw}) - \frac{\me^2 (1 + z)^2}{\Delw} }.
	}
	With Eq.~\refeq{delZqq}, we find
	\ans{\al{
		\del\Zq &= \intoq \ddz (1 - z) \left\{ \frac{\lam^2}{64 \pi^2} \brac{ \frac{4}{\eps} - 1 - 2 \gam + 2 \ln(\frac{4 \pi}{\Delw}) - \frac{\me^2 (1 + z)^2}{\Delw} } \right. \\
		&\hspace{15em} \phantom{=\ } \left. - \frac{e^2}{8 \pi^2} \brac{ \frac{4}{\eps} - 2 - 2 \gam + 2 \ln(\frac{4\pi}{\Delq}) - \frac{\me^2 (z^2 - z + 1)}{\Delq} } \right\}.
	}}%
	
	For $\del\Zw$, we need to add the loop diagrams of a photon and a scalar.  We calculated the former in \ref{1b} and the latter in \ref{2a}.  Applying Eqs.~\refeq{Zw1b} and \refeq{Zw2a}, we have
	\ans{\al{
		\del\Zw &= \intoq \ddx \left\{ \frac{\lam^2}{32 \pi^2} x \brac{ -\frac{2}{\eps} + \gam - \ln(\frac{4\pi}{\Delw}) - \frac{2 \me^2 (1 + x) (1 - x)}{\Delw} } \right. \\
		&\hspace{10em} \phantom{=\ } \left. - \frac{e^2}{16 \pi^2} (1 - x) \brac{ \frac{4}{\eps} - 5 - 2 \gam + 2 \ln(\frac{4\pi}{\Delq}) - \frac{m^2 (1 - 2x - x^2)}{\Delq} } \right\}.
	}}%
	where $\Delq = (1 - z)^2 m^2 + z \mu^2$ and $\Delw = (1 - z)^2 \me^2 + z \mphi^2$.  It certainly appears that $\del\Zq \neq \del\Zw$ in this case, but I am not sure whether this is because I actually computed each correctly.
}