\newcommand{\vr}{\vec{r}}

\newcommand{\Li}{L_i}
\newcommand{\Lx}{L_x}
\newcommand{\Ly}{L_y}
\newcommand{\Lz}{L_z}
\newcommand{\Lw}{L^2}

\newcommand{\Px}{P_x}
\newcommand{\Py}{P_y}
\newcommand{\Pz}{P_z}

\newcommand{\Ri}{R_i}
\newcommand{\Rx}{R_x}
\newcommand{\Ry}{R_y}
\newcommand{\Rz}{R_z}

\newcommand{\Rit}{\Ri(\theta)}
\newcommand{\Rxt}{\Rx(\theta)}
\newcommand{\Ryt}{\Ry(\theta)}
\newcommand{\Rzt}{\Rz(\theta)}

\newcommand{\cost}{\cos{\theta}}
\newcommand{\sint}{\sin{\theta}}

\newcommand{\Mi}{M_i}
\newcommand{\Mx}{M_x}
\newcommand{\My}{M_y}
\newcommand{\Mz}{M_z}

\newcommand{\Jpm}{J_\pm}
\newcommand{\Jp}{J_+}
\newcommand{\Jm}{J_-}

\newcommand{\veps}{\varepsilon}
\newcommand{\hbsqt}{\frac{\hbar}{\sqrt{2}}}

\section{Problem 3}
\begin{statement}
	Answer the following questions about the angular momentum operator $\Li$.
\end{statement}

\begin{problem}
	Calculate $[\Li, \vr]$ where $i = x, y, z$.
\end{problem}

\begin{solution}
	Firstly, note that
	\begin{align*}
		\Lx &= Y \Pz - Z \Py, &
		\Ly &= Z \Px - X \Pz, &
		\Lz &= X \Py - Y \Px,
	\end{align*}
	where the expression for $\Lz$ was given in problem 2 of Homework 1, and $\Lx$ and $\Ly$ are cyclic permutations.  Then
	\begin{align*}
		[\Lx, X] &= (Y \Pz - Z \Py) X - X (Y \Pz - Z \Py) = 0, \\
		[\Lx, Y] &= (Y \Pz - Z \Py) Y - Y (Y \Pz - Z \Py) = Y \Pz Y - Z \Py Y - Y Y \Pz + Y Z \Py = [Y, \Py] Z = \ihb Z, \\
		[\Lx, Z] &= (Y \Pz - Z \Py) Z - Z (Y \Pz - Z \Py) = Y \Pz Z - Z \Py Z - Z Y \Pz + Z Z \Py = -[Z, \Pz] Y = -\ihb Y.
	\end{align*}
	Generalizing these results to $\Ly$ and $\Lz$,
	\begin{align*}
		[\Lx, \vr] &= \ihb \mqty[ 0 \\ Z \\ -Y ], &
		[\Ly, \vr] &= \ihb \mqty[ -Z \\ 0 \\ X ], &
		[\Lz, \vr] &= \ihb \mqty[ Y \\ -X \\ 0 ],
	\end{align*}
	where $\vr = \mqty[X & Y & Z]^T$.
\end{solution}

\begin{problem}
	Let us now compare the above results with classical mechanics.  Rotations around the $x$, $y$, and $z$ axes by an angle $\theta$ in three-dimensional Cartesian space are represented by the following matrices:
	\begin{align*}
		\Rxt &= \mqty[ 1 & 0 & 0 \\ 0 & \cost & -\sint \\ 0 & \sint & \cost ], &
		\Ryt &= \mqty[ \cost & 0 & \sint \\ 0 & 1 & 0 \\ -\sint & 0 & \cost ], &
		\Rzt &= \mqty[ \cost & -\sint & 0 \\ \sint & \cost & 0 \\ 0 & 0 & 1 ].
	\end{align*}
	Calculate $\Rit \, \vr$.  Then expand $\Rit \, \vr$ for a small angle $\theta$ and consider $\vr - \Rit \, \vr$ to first order in $\theta$,
	\beq
		\vr - \Rit \, \vr = \theta \Mi \vr + \order{\theta^2}.
	\eeq
	Calculate the matrices $\Mi$.
\end{problem}

\begin{solution}
	For $\Rit \, \vr$, we have
	\begin{align*}
		\Rxt \, \vr &= \mqty[ X \\ \cost Y - \sint Z \\ \sint Y + \cost Z ], &
		\Ryt \, \vr &= \mqty[ \cost X + \sint Z \\ Y \\ \cost Z - \sint X ], &
		\Rzt \, \vr &= \mqty[ \cost X - \sint Y \\ \sint X + \cost Y \\ Z ],
	\end{align*}
	In the small angle approximation, to first order $\cost \approx 1$ and $\sint \approx \theta$.  In this approximation,
	\begin{align*}
		\Rxt \, \vr &\approx \mqty[ X \\ Y - \theta Z \\ \theta Y + Z ], &
		\Ryt \, \vr &\approx \mqty[ X + \theta Z \\ Y \\ Z - \theta X ], &
		\Rzt \, \vr &\approx \mqty[ X - \theta Y \\ \theta X + Y \\ Z ],
	\end{align*}
	and so
	\begin{align*}
		\vr - \Rxt \, \vr &\approx \mqty[ 0 \\ \theta Z \\ -\theta Y ], &
		\vr - \Ryt \, \vr &\approx \mqty[ -\theta Z \\ 0 \\ \theta X ], &
		\vr - \Rzt \, \vr &\approx \mqty[ \theta Y \\ -\theta X \\ 0 ].
	\end{align*}
	These results suggest the matrices
	\begin{align*}
		\Mx &= \mqty[ 0 & 0 & 0 \\ 0 & 0 & 1 \\ 0 & -1 & 0 ], &
		\My &= \mqty[ 0 & 0 & -1 \\ 0 & 0 & 0 \\ 1 & 0 & 0 ], &
		\Mz &= \mqty[ 0 & 1 & 0 \\ -1 & 0 & 0 \\ 0 & 0 & 0 ].
	\end{align*}
\end{solution}

\newcommand{\klm}{\ket{l, m}}

\begin{problem}
	Calculate the matrix elements of the angular momentum operator $\Li$ in the basis ket $\klm$ when $l = 1$ and $l = 2$.  Here, $\klm$ is the simultaneous eigenket of $\Lw$ and $\Lz$ with the eigenvalues $\hbar^2 l (l + 1)$ and $\hbar m$, respectively.
\end{problem}

\begin{solution}
	The ladder operators are defined by (3.5.5) in Sakurai:
	\beq
		\Jpm = \Lx \pm i \Ly.
	\eeq
	Clearly,
	\begin{align*}
		\Lx &= \frac{\Jp + \Jm}{2}, &
		\Ly &= \frac{\Jp - \Jm}{2 i}
	\end{align*}
	From (3.5.39) and (3.5.40),
	\begin{align*}
		\Jp \klm &= \sqrt{(l - m)(l + m + 1)} \hbar \ket{l, m+1}, &
		\Jm \klm &= \sqrt{(l + m)(l - m + 1)} \hbar \ket{l, m-1}.
	\end{align*}
	
	Then the matrix elements of $\Lx$ are given by
	\begin{align*}
		\mel*{1, m'}{\Lx}{1, m} &= \mel*{1, m'}{\frac{\Jp + \Jm}{2}}{1, m} = \frac{\hbar}{2} \left( \delta_{m+1, m'} \sqrt{2 - m - m^2} + \delta_{m-1, m'} \sqrt{2 + m - m^2} \right), \\
		\mel*{1, m'}{\Lx}{2, m} &= 0, \\
		\mel*{2, m'}{\Lx}{1, m} &= 0, \\
		\mel*{2, m'}{\Lx}{2, m} &= \mel*{1, m'}{\frac{\Jp + \Jm}{2}}{1, m} = \frac{\hbar}{2} \left( \delta_{m+1, m'} \sqrt{6 - m - m^2} + \delta_{m-1, m'} \sqrt{6 + m - m^2} \right),
	\end{align*}
	where the integers $m, m' \in [-l, l]$.
	
	The matrix elements of $\Ly$ are given by
	\begin{align*}
		\mel*{1, m'}{\Ly}{1, m} &= \mel*{1, m'}{\frac{\Jp - \Jm}{2 i}}{1, m} = -\frac{\ihb}{2} \left( \delta_{m+1, m'} \sqrt{2 - m - m^2} - \delta_{m-1, m'} \sqrt{2 + m - m^2} \right), \\
		\mel*{1, m'}{\Ly}{2, m} &= 0, \\
		\mel*{2, m'}{\Ly}{1, m} &= 0, \\
		\mel*{2, m'}{\Ly}{2, m} &= \mel*{1, m'}{\frac{\Jp - \Jm}{2 i}}{1, m} = -\frac{\ihb}{2} \left( \delta_{m+1, m'} \sqrt{6 -m - m^2} - \delta_{m-1, m'} \sqrt{6 + m - m^2} \right),
	\end{align*}
	where again $m, m' \in [-l, l]$.
		
	Since $\klm$ are eigenkets of $\Lz$, its matrix elements are given by
	\beq
		\mel*{l', m'}{\Ly}{l, m} = \hbar m \, \delta_{m, m'} \, \delta_{l, l'},
	\eeq
	where $l, l' \in \{1, 2\}$ and $m, m' \in [-l, l]$.
	
	Explicitly, let
	\beq
		R = \kbordermatrix{ & (1, -1) & (1, 0) & (1, 1) & (2, -2) & (2, -1) & (2, 0) & (2, 1) & (2, 2) \cr
				(1, -1) & 0 & 1 & 0 & 0 & 0 & 0 & 0 & 0 \cr
				(1, 0) & 1 & 0 & 1 & 0 & 0 & 0 & 0 & 0 \cr
				(1, 1) & 0 & 1 & 0 & 0 & 0 & 0 & 0 & 0 \cr
				(2, -2) & 0 & 0 & 0 & 0 & \sqrt{2} & 0 & 0 & 0 \cr
				(2, -1) & 0 & 0 & 0 & \sqrt{2} & 0 & \sqrt{3} & 0 & 0 \cr
				(2, 0) & 0 & 0 & 0 & 0 & \sqrt{3} & 0 & \sqrt{3} & 0 \cr
				(2, 1) & 0 & 0 & 0 & 0 & 0 & \sqrt{3} & 0 & \sqrt{2} \cr
				(2, 2) & 0 & 0 & 0 & 0 & 0 & 0 & \sqrt{2} & 0 \cr
			},
	\eeq
	where the row labels represent $(l', m')$ and the column labels represent $(l, m)$.  Then
	\begin{align*}
		\Lx &= \frac{\hbar}{\sqrt{2}} R, &
		\Ly &= -\frac{\ihb}{\sqrt{2}} R,
	\end{align*}
	and
	\beq
		\Lz = \hbar \kbordermatrix{ & (1, -1) & (1, 0) & (1, 1) & (2, -2) & (2, -1) & (2, 0) & (2, 1) & (2, 2) \cr
				(1, -1) & -1 & 0 & 0 & 0 & 0 & 0 & 0 & 0 \cr
				(1, 0) & 0 & 0 & 0 & 0 & 0 & 0 & 0 & 0 \cr
				(1, 1) & 0 & 0 & 1 & 0 & 0 & 0 & 0 & 0 \cr
				(2, -2) & 0 & 0 & 0 & -2 & 0 & 0 & 0 & 0 \cr
				(2, -1) & 0 & 0 & 0 & 0 & -1 & 0 & 0 & 0 \cr
				(2, 0) & 0 & 0 & 0 & 0 & 0 & 0 & 0 & 0 \cr
				(2, 1) & 0 & 0 & 0 & 0 & 0 & 0 & 1 & 0 \cr
				(2, 2) & 0 & 0 & 0 & 0 & 0 & 0 & 0 & 2 \cr
			}.
	\eeq
\end{solution}