\documentclass[11pt]{article}
\usepackage{homework}

\usepackage{slashed}

\classname{443}
\homeworknum{6}


\begin{document}

\input{definitions}
\input{probdefs}


\state{Exotic contributions to $\mathbf{g - 2}$~(Peskin \& Schroeder~6.3)}{
	Any particles that couples to the electron can produce a correction to the electron-photon form factors and, in particular, a correction to $g - 2$.  Because the electron $g - 2$ agrees with QED to high accuracy, these corrections allow us to constrain the properties of hypothetical new particles.
}

\prob{ \label{1a}
	The unified theory of weak and electromagnetic interactions contains a scalar particle $h$ called the \emph{Higgs boson}, which couples to the electron according to
	\eq{
		\Hint = \int \ddcx \frac{\lam}{\sqrt{2}} h \psib \psi.
	}
	Compute the contribution of a virtual Higgs boson to the electron $(g - 2)$, in terms of $\lam$ and the mass $\mh$ of the Higgs boson.
}

\sol{
	We are interested in the diagram
	\eqn{diag}{
		\centergraphics{diag/loop}
	}
	The Higgs field is a scalar Yukawa field, so we can use the form of the Yukawa interaction Hamiltonian of Peskin \& Schroeder~(4.112) and the appropriate Feynman rules to write~\cite[p.~118]{Peskin}
	\al{
		\centergraphics{diag/vertex} &= -i \frac{\lam}{\sqrt{2}}, &
		\centergraphics{diag/propagator} &= \frac{i}{q^2 - \mh^2 + i \eps}.
	}
	Our diagram is similar to the one on p.~189 in Peskin \& Schroeder.  We can then adapt (6.38) to write
	\aln{
		\ubpp \del\Gammppp \up &= \int \ddqkf \frac{i}{(k - p)^2 - \mh^2 + i \eps} \ubpp \paren{ -i \frac{\lam}{\sqrt{2}} } \frac{i (\ksl' + \me)}{{k'}^2 - \me^2 + i \eps} \gamm \frac{i (\ksl + \me)}{k^2 - \me^2 + i \eps} \paren{ -i \frac{\lam}{\sqrt{2}} } \up \notag \\
		&= i \frac{\lam^2}{2} \int \ddqkf \ubpp \frac{(\ksl' + \me) \gamm (\ksl + \me)}{[ (k - p)^2 - \mh^2 + i \eps ] ({k'}^2 - \me^2 + i \eps) (k^2 - \me^2 + i \eps)} \up. \label{thing1a}
	}
	To evaluate the integral, we use Peskin \& Schroeder~(6.41) with $n = 3$:
	\eq{
		\frac{1}{\Aq \Aw \cdots \An} = \intoq \ddxq \cdots \ddxn \del\paren{ \sum \xii - 1 } \frac{(n - 1)!}{(\xq \Aq + \xw \Aw + \cdots + \xn \An)^n}.
	}
	Applying this to the denominator of the integrand of Eq.~\refeq{thing1a} gives us
	\eqn{denom}{
		\frac{1}{[ (k - p)^2 - \mh^2 + i \eps ] ({k'}^2 - \me^2 + i \eps) (k^2 - \me^2 + i \eps)} = \intoq \ddx \ddy \ddz \del(x + y + z - 1) \frac{2}{D^3},
	}
	where~\cite[pp.~190--191]{Peskin}
	\al{
		D &= x (k^2 - \me^2) + y ({k'}^2 - \me^2) + z [ (k - p)^2 - \mh^2 ] + (x + y + z) i \eps \\
		&= x (k^2 - \me^2) + y (k^2 + 2 k q + q^2 - \me^2) + z (k^2 - 2 k p + p^2 - \mh^2) + i \eps \\
		&= (x + y + z) k^2 - (x + y) \me^2 + 2 k (q y - p z) + z (p^2 - \mh^2) + i \eps \\
		&= k^2 + 2 k (q y - p z) + z (p^2 - \mh^2) - (1 - z) \me^2 + i \eps.
	}
	Here we have used $x + y + z = 1$ and $k' = k + q$.  Let $\ell \equiv k + y q - z p$~\cite[p.~191]{Peskin}.  Then
	\eqn{D}{
		D = \ell^2 + x y q^2 - (1 - z)^2 \me^2 - \mh^2 z + i \eps
		\equiv \ell^2 - \Del + i \eps,
	}
	where we have defined $\Del \equiv -x y q^2 + (1 - z)^2 \me^2 + z \mh^2$~\cite[p.~191]{Peskin}.
	
	For the numerator of Eq.~\refeq{thing1a}, let $N \equiv \ubpp (\ksl' + \me) \gamm (\ksl + \me) \up$.  Then using $k' = k + q$ and $\ell \equiv k + y q - z p$~\cite[p.~191]{Peskin},
	\eqn{N1}{
		N = \ubpp (\ksl + \qsl + \me) \gamm (\ksl + \me) \up
		= \ubpp [ \lsl + (1 - y) \qsl + z \psl + \me ] \gamm (\lsl - y \qsl + z \psl + \me) \up.
	}
	We should be able to write this as an expression of the form given in (6.31) of Peskin \& Schroeder~\cite[p.~191]{Peskin},
	\eqn{ABC}{
		\Gamm = \gamm \cdot A + ({\pmm}' + \pmm) \cdot B + ({\pmm}' - \pmm) \cdot C
		= \gamm \cdot A + ({\pmm}' + \pmm) \cdot B + \qm \cdot C.
	}
	But from (6.45),
	\eq{
		\int \ddqlf \frac{\lm}{D^3} = 0.
	}
	This means we can discard terms of $\order{\ell}$.  We also know from (6.33) that
	\eqn{Gam}{
		\Gammppp = \gamm \Fqqs + \frac{i \sigmn \qsn}{2 \me} \Fwqs.
	}
	Since the correction to $g - 2$ is given by $\Fwqso = 0 + \del\Fwqso$ (since $\Fw = 0$ to lowest order), we can discard terms of $\order{\gamm}$ in Eq.~\refeq{N1}~\cite[pp.~186, 196]{Peskin}.  So Eq.~\refeq{N1} becomes
	\aln{
		N &= \ubpp [ \lsl + (1 - y) \qsl + z \psl + \me ] \gamm (\lsl - y \qsl + z \psl + \me) \up \notag \\[1ex]
		&= \ubpp [ \lsl \gamm \lsl - y (1 - y) \qsl \gamm \qsl + z (1 - y) \qsl \gamm \psl + \me (1 - y) \qsl \gamm - y z \psl \gamm \qsl \notag \\
		&\hspace{20em} \phantom{=\ } + z^2 \psl \gamm \psl + \me z \psl \gamm - \me y \gamm \qsl + \me z \gamm \psl ] \up. \label{N2}
	}
	To simplify these terms, we use Peskin \& Schroeder~(6.46):
	\eq{
		\int \ddqlf \frac{\lmm \lnn}{D^3} = \int \ddqlf \frac{\gmn \ell^2}{4 D^3},
	}
	as well as~\cite[pp.~191--192]{Peskin}
	\al{
		\psl \gamm &= 2 \pmm - \gamm \psl, &
		\psl \up &= \me \up, &
		\ubpp \psl' &= \ubpp \me
	}
	and~\cite{Gamma, Feynman}
	\al{
		\asl \bsl &= a \cdot b, &
		\asl \bsl + \bsl \asl = 2 a \cdot b.
	}
	We find
	\al{
		\lsl \gamm \lsl &= (2 \lm - \gamm \lsl) \lsl
		= 2 \lm \lnn \gamsn - \gamm \lsl \lsl
		\to \frac{\ell^2 \gmn \gamsn}{2} - \gamm \ell^2
		= -\frac{\ell^2 \gamm}{2} \\
		&\to 0,
		\\[1ex]
		\qsl \gamm \qsl &= (2 \qm - \gamm \qsl) \qsl
		\to - \gamm \qsl \qsl
		= -q^2 \gamm \\
		&\to 0,
		\\[1ex]
		\qsl \gamm \psl &\to \qsl \gamm \me
		= (\psl' - \psl) \gamm \me
		\to (\me - \psl) \gamm \me
		= \me^2 \gamm - 2 \me \pmm + \me \gamm \psl \\
		&\to -2 \me \pmm,
		\\[1ex]
		\qsl \gamm &= (\psl' - \psl) \gamm
		\to \me \gamm - \psl \gamm
		\to -2 \pmm + \gamm \psl
		\to -2 \pmm + \gamm \me \\
		&\to -2 \pmm,
		\\[1ex]
		\psl \gamm \qsl &= (2 \pmm - \gamm \psl) \qsl
		\to -\gamm \psl \qsl
		= -2 \gamm p \cdot q + \gamm \qsl \psl
		\to -2 \gamm p \cdot q + \gamm (\psl' - \psl) \me \\
		&\to \gamm q^2 + \me \gamm \psl' - \me^2 \gamm
		= \gamm q^2 + \me (2 {\pmm}' - \psl' \gamm) - \me^2 \gamm
		\to \gamm q^2 + 2 \me {\pmm}' - 2 \me^2 \gamm \\
		&\to 2 \me {\pmm}',
	}
		where we have used
	\eq{
		2 p \cdot q = p \cdot q + q \cdot p
		= p \cdot q + p' \cdot q - q^2
		= {p'}^2 + p' \cdot p - p' \cdot p - p^2 - q^2
		\to \me^2 - \me^2 - q^2
		= -q^2,
	}
	and
	\al{
		\psl \gamm \psl &\to \me \psl \gamm
		= \me (2 \pmm - \gamm \psl)
		\to 2 \me \pmm - \me^2 \gamm
		\to 2 \me \pmm,
		\\[1ex]
		\psl \gamm &= 2 \pmm - \gamm \psl
		= 2 \pmm - \gamm \me
		\to 2 \pmm,
		\\[1ex]
		\gamm \qsl &= \gamm (\psl' - \psl)
		\to \gamm \psl' - \gamm \me
		\to 2 {\pmm}' - \psl' \gamm
		\to 2 {\pmm}' - \me \gamm
		\to 2 {\pmm}',
		\\[1ex]
		\gamm \psl &\to 0.
	}
	Feeding these into Eq.~\refeq{N2}, we obtain
	\aln{
		N &= \ubpp [ - 2 \me z (1 - y) \pmm - 2 \me (1 - y) \pmm - 2 \me y z {\pmm}' + 2 \me z^2 \pmm + 2 \me z \pmm - 2 \me y {\pmm}' ] \up \notag \\
		&= 2 \me \ubpp \{ [ z^2 + z - z (1 - y) - (1 - y) ] \pmm - y (1 + z) {\pmm}' \} \up \notag \\
		&= 2 \me \ubpp \{ [ z^2 + y (1 + z) - 1 ] \pmm - y (1 + z) {\pmm}' \} \up \notag \\
		&= 2 \me \ubpp [ (z^2 - 1) \pmm + y (1 + z) (\pmm - {\pmm}') ] \up \notag \\
		&= \me \ubpp [ (z^2 - 1) \pmm + (z^2 - 1) \pmm + 2 y (1 + z) (\pmm - {\pmm}') + (z^2 - 1) {\pmm}' - (z^2 - 1) {\pmm}' ] \up \notag \\
		&= \me \ubpp [ (z^2 - 1) (\pmm + {\pmm}') + (z^2 - 1) (\pmm - {\pmm}') + 2 y (1 + z) (\pmm - {\pmm}') ] \up \notag \\
		&= \me \ubpp [ (z^2 - 1) (\pmm + {\pmm}') - (z^2 + 2 y (1 + z) - 1) ({\pmm}' - \pmm) ] \up, \label{N3}
	}
	which has the form of the second two terms of Eq.~\refeq{ABC}.  According to the Ward identity, the coefficient of $\qm = {\pmm} - \pmm$ vanishes~\cite[p.~192]{Peskin}.  Further, according to the Gordon identity given by Peskin \& Schroeder~(6.32),
	\eq{
		\ubpp \gamm \up = \ubpp \paren{ \frac{{\pmm}' + \pmm}{2 m} + \frac{i \sigmn \qsn}{2 m} } \up.
	}
	So Eq.~\refeq{N3} becomes
	\eqn{N4}{
		N = i \me \ubpp (1 - z^2) \sigmn \gmn \up.
	}
	Feeding Eqs.~\refeq{denom}, \refeq{D}, and \refeq{N4} into Eq.~\refeq{thing1a}, we have (ignoring the $\order{\gamm}$ term)
	\eq{
		\ubpp \del\Gammppp \up \to i \frac{\lam^2}{2} \int \ddqlf \intoq \ddx \ddy \ddz \del(x + y + z - 1) \ubpp \frac{2 i \me (1 - z^2) \sigmn \gmn}{(\ell^2 - \Del + i \eps)^3} \up.
	}
	From Eq.~\refeq{Gam}, we can write
	\eq{
		\del\Fwqs = i \frac{\lam^2}{2} \int \ddqlf \intoq \ddx \ddy \ddz \del(x + y + z - 1) \frac{2 \me^2 (1 - z^2)}{(\ell^2 - \Del + i \eps)^3}.
	}
	Computing the integral using Peskin \& Schroeder~(6.49),
	\eqn{6.49}{
		\int \ddqlf \frac{1}{(\ell^2 - \Del)^m} = \frac{i (-1)^m}{(4\pi)^2} \frac{1}{(m - 1) (m - 2)} \frac{1}{\Del^{m - 2}},
	}
	we find
	\eq{
		\del\Fwqs = \frac{\lam^2}{(4\pi)^2} \intoq \ddx \ddy \ddz \del(x + y + z - 1) \frac{\me^2 (1 - z^2)}{\Del}.
	}
	So, using Eq.~\refeq{D},
	\al{
		\del\Fwqso &= \frac{\lam^2}{(4\pi)^2} \intoq \ddx \ddy \ddz \del(x + y + z - 1) \frac{\me^2 (1 - z^2)}{(1 - z)^2 \me^2 + z \mh^2} \\
		&= \frac{\lam^2}{(4\pi)^2} \intoq \ddz \int_0^{1 - z} \ddy \frac{\me^2 (1 - z^2)}{(1 - z)^2 \me^2 + z \mh^2} \\
		&= \frac{\lam^2}{(4\pi)^2} \intoq \ddz \frac{\me^2 (1 - z^2) (1 - z)}{(1 - z)^2 \me^2 + z \mh^2} \\
		&= \frac{\lam^2 \me^2}{(4\pi)^2} \intoq \ddz \frac{1 - z - z^2 + z^3}{(1 - z)^2 \me^2 + z \mh^2} \\
		&= \frac{\lam^2 \me^2}{(4\pi)^2} \paren{ \intoq \ddz \frac{1}{(1 - z)^2 \me^2 + z \mh^2} - \intoq \ddz \frac{z (1 + z - z^2)}{(1 - z)^2 \me^2 + z \mh^2} } \\
		&\approx \frac{\lam^2}{(4\pi)^2} \frac{\me^2}{\mh^2} \paren{ \int_{\me^2}^{\mh^2} \frac{\ddu}{u} - \intoq \ddz (1 + z - z^2) } \\
		&= \frac{\lam^2}{(4\pi)^2} \frac{\me^2}{\mh^2} \paren{ \bigg[ \ln u \bigg]_{\me^2}^{\mh^2} - \brac{ z + \frac{z^2}{2} - \frac{z^3}{3} }_0^1 },
	}
	where we have used the substitution $u = (1 - z)^2 \me^2 + z \mh^2$, and
	\eq{
		\ddu = 2 (z - 1) \me^2 + \mh^2
		\approx \mh^2
	}
	in the limit $\me \ll \mh$.  Referring to Peskin \& Schroeder~(6.58) and (6.59), we have
	\eqn{a}{
		\ans{ \Fwqso = \frac{\lam^2}{(4\pi)^2} \frac{\me^2}{\mh^2} \brac{ \ln(\frac{\mh^2}{\me^2}) - \frac{7}{6} } }
	}
	as the correction to the electron $g$ factor from a virtual Higgs boson.
}



\prob{
	QED accounts extremely well for the electron's anomalous magnetic moment.  If $a = (g - 2) / 2$,
	\eq{
		\abs{\aexpt - \aQED} < \num{1e-10}.
	}
	What limits does this place on $\lam$ and $\mh$?  In the simplest version of the electroweak theory, $\lam = \num{3e-6}$ and $\mh > \SI{60}{\GeV}$.  Show that these values are not excluded.  The coupling of the Higgs boson to the muon is larger by a factor $(\mmu / \me)$: $\lam = \num{6e-4}$.  Thus, although our experimental knowledge of the muon anomalous magnetic moment is not as precise,
	\eq{
		\abs{\aexpt - \aQED} < \num{3e-8},
	}
	one can still obtain a stronger limit on $\mh$.  Is it strong enough?
}

\sol{
	Feeding $\me = \meSI$ into Eq.~\refeq{a}, the limit becomes
	\eq{
		\frac{\lam^2}{\mh^2} \brac{ \ln(\frac{\mh^2}{\meSIs}) - \frac{7}{6} } < \SI{6.05e-8}{\per\square\MeV}.
	}
	For $\lam = \num{3e-6}$ and $\mh > \SI{60}{\GeV}$,
	\eq{
		\abs{\aexpt - \aQED} < \frac{(\num{3e-6})^2}{(4\pi)^2} \frac{(\meSI)^2}{(\mhSI)^2} \brac{ \ln(\frac{(\mhSI)^2}{(\meSI)^2}) - \frac{7}{6} }
		\approx \ans{ \num{9e-23} < \num{1e-10}, }
	}
	so these values are not excluded. \qed
	
	Now using $\lam = \num{6e-4}$ and $\mmu = \mmuSI$~\cite{PDG},
	\eq{
		\abs{\aexpt - \aQED} < \frac{(\num{6e-4})^2}{(4\pi)^2} \frac{(\mmuSI)^2}{(\mhSI)^2} \brac{ \ln(\frac{(\mhSI)^2}{(\mmuSI)^2}) - \frac{7}{6} }
		\approx \ans{ \num{8e-14} < \num{1e-10}, }
	}
	so these values are not excluded either, although they come closer to the upper limit.
}



\prob{
	Some more complex versions of this theory contain a pseudoscalar particle called the \emph{axion}, which couples to the electron according to
	\eq{
		\Hint = \int \ddcx \frac{i \lam}{\sqrt{2}} a \psib \gamt \psi.
	}
	The axion may be as light as the electron, or lighter, and may couple more strongly than the Higgs boson.  Compute the contribution of a virtual axion to the $g - 2$ of the electron, and work out the excluded values of $\lam$ and $\ma$.
}

\sol{
	The diagram we are interested in is the same as Eq.~\refeq{diag}, but now the dashed line represents the pseudoscalar axion rather than the scalar Higgs boson.  The Feynman rules are now~\cite[pp.~24--25]{Axion}
	\al{
		\centergraphics{diag/vertex} &= \frac{\lam}{\sqrt{2}} \gamt, &
		\centergraphics{diag/propagator} &= \frac{i}{q^2 - \mh^2 + i \eps}.
	}
	Again, we adapt Peskin \& Schroeder~(6.38) to write
	\aln{
		\ubpp \del\Gammppp \up &= \int \ddqkf \frac{i}{(k - p)^2 - \mh^2 + i \eps} \ubpp \paren{ \frac{\lam}{\sqrt{2}} \gamt } \frac{i (\ksl' + \me)}{{k'}^2 - \me^2 + i \eps} \gamm \frac{i (\ksl + \me)}{k^2 - \me^2 + i \eps} \paren{ \frac{\lam}{\sqrt{2}} \gamt } \up \notag \\
		&= i \frac{\lam^2}{2} \int \ddqkf \ubpp \frac{\gamt (\ksl' + \me) \gamm (\ksl + \me) \gamt}{[ (k - p)^2 - \mh^2 + i \eps ] ({k'}^2 - \me^2 + i \eps) (k^2 - \me^2 + i \eps)} \up. \label{thing1c}
	}
	The denominator is the same as in \ref{1a}.  For the numerator, 
	\al{
		N &= \ubpp \gamt (\ksl' + \me) \gamm (\ksl + \me) \gamt \up \\
		&= \ubpp (-\ksl' + \me) \gamm (-\ksl + \me) \up \\
		&= -\ubpp (\ksl' - \me) \gamm (\ksl - \me) \up
	}
	since $\{ \gamt, \gamm \} = 0$ and $(\gamt)^2 = 1$ by Peskin \& Schroeder~(3.70) and (3.71).  Feeding in $k' = k + q$ and $\ell \equiv k + y q - z p$, and using the calculations from \ref{1a},
	\al{
		N &= -\ubpp [ \lsl + (1 - y) \qsl + z \psl - \me ] \gamm (\lsl - y \qsl + z \psl - \me) \up \\[1ex]
		&= -\ubpp [ \lsl \gamm \lsl - y (1 - y) \qsl \gamm \qsl + z (1 - y) \qsl \gamm \psl - \me (1 - y) \qsl \gamm - y z \psl \gamm \qsl \\
		&\hspace{20em} \phantom{=\ } + z^2 \psl \gamm \psl - \me z \psl \gamm + \me y \gamm \qsl - \me z \gamm \psl ] \up \\[1ex]
		&\to -\ubpp [ -2 \me z (1 - y) \pmm + 2 \me (1 - y) \pmm - 2 \me y z {\pmm}' + 2 \me z^2 \pmm - 2 \me z \pmm + 2 \me y {\pmm}' ] \up \\[1ex]
		&= -2 \me \ubpp \{ [ (1 - z)^2 - y (1 - z) ] \pmm + y (1 - z) {\pmm}' \} \up \\[1ex]
		&= -2 \me \ubpp [ (1 - z)^2 \pmm + y (1 - z) ({\pmm} - \pmm) ] \up \\[1ex]
		&= -\me \ubpp [ (1 - z)^2 \pmm + (1 - z)^2 \pmm + (1 - z)^2 {\pmm}' - (1 - z)^2 {\pmm}' + 2 y (1 - z) ({\pmm}' - \pmm) ] \up \\[1ex]
		&= -\me \ubpp [ (1 - z)^2 (\pmm + {\pmm}') - (1 - z)^2 ({\pmm}' - \pmm) + 2 y (1 - z) ({\pmm}' - \pmm) ] \up \\[1ex]
		&= \me \ubpp [ (z - 1) (2 y + z - 1) ({\pmm}' - \pmm) - (1 - z)^2 (\pmm + {\pmm}') ] \up.
	}
	Feeding this as well as Eqs.~\refeq{denom} and \refeq{D} into Eq.~\refeq{thing1a}, we have (again ignoring the $\order{\gamm}$ term)
	\eq{
		\ubpp \del\Gammppp \up \to i \frac{\lam^2}{2} \int \ddqlf \intoq \ddx \ddy \ddz \del(x + y + z - 1) \ubpp \frac{2 i \me (1 - z)^2 \sigmn \gmn}{(\ell^2 - \Del + i \eps)^3} \up.
	}
	Once again using Eq.~\refeq{6.49}, we find
	\eq{
		\del\Fwqs = \frac{\lam^2}{(4\pi)^2} \intoq \ddx \ddy \ddz \del(x + y + z - 1) \frac{\me^2 (1 - z)^2}{\Del},
	}
	which implies
	\al{
		\del\Fwqso &= \frac{\lam^2}{(4\pi)^2} \intoq \ddx \ddy \ddz \del(x + y + z - 1) \frac{\me^2 (1 - z)^2}{(1 - z)^2 \me^2 + z \ma^2} \\
		&= \frac{\lam^2}{(4\pi)^2} \intoq \ddz \int_0^{1 - z} \ddy \frac{\me^2 (1 - z)^2}{(1 - z)^2 \me^2 + z \ma^2} \\
		&= \frac{\lam^2 \me^2}{(4\pi)^2} \intoq \ddz \frac{(1 - z)^3}{(1 - z)^2 \me^2 + z \ma^2}.
	}
	In the limit $\ma \ll \me$, which is consistent with current limits on axion masses~\cite{PDG}
	\eq{
		\del\Fwqso \approx \frac{\lam^2 \me^2}{(4\pi)^2} \intoq \ddz \frac{(1 - z)^3}{(1 - z)^2 \me^2}
		= \frac{\lam^2}{(4\pi)^2} \intoq \ddz (1 - z)
		= \frac{\lam^2}{(4\pi)^2} \bigg[ 1 - \frac{z^2}{2} \bigg]
		= \ans{ \frac{\lam^2}{32 \pi^2} }
	}
	is the contribution of a virtual axion to the electron $g - 2$.  For the excluded values of $\lam$, then,
	\eq{
		\frac{\lam^2}{32 \pi^2} < \num{1e-10}
		\qimplies \lam < \num{1.78e-4}.
	}
	This means \ans{$\lam > \num{1.78e-4}$} is excluded for $\ma \ll \me$.
}


\makebib

\end{document}
