\begin{statement}{}
	The angular momentum density of the electromagnetic field is given by
	\beq
		\vl = \vx \times \vcP
		= \frac{c}{4\pi} \vx \times (\vE \times \vB).
	\eeq
	Consider a source free ($\rho = 0$, $\vJ = 0$) solution to Maxwell's equations in electrodynamics with $\vE$ and $\vB$ vanishing rapidly as $\absx \to \infty$, so the total angular momentum
	\beq
		\vL = \int \vl \dcx
	\eeq
	is well defined.  Show that $\vL$ is conserved, i.e., independent of time.
\end{statement}

\begin{solution}
	We want to show that
	\beq
		\dv{\vL}{t} = 0.
	\eeq
	From Eq.~(5.18), the failure of linear momentum conservation to hold for the electromagnetic field alone, in general, is
	\beq
		\pdv{\cPi}{t} - \sum_{j=1}^3 \partial_j \Tij = - \left[ \rho \Ei + \frac{1}{c} (\vJ \times \vB)_i \right],
	\eeq
	where the stress-energy tensor $\Tij$ is defined in Eq.~(5.11),
	\beq
		\Tij = \frac{1}{4\pi} \left[ \Ei \Ej + \Bi \Bj - \frac{1}{2} \delij (\abs{\vE}^2 + \abs{\vB}^2) \right],
	\eeq
	and Eq.~(5.19) defines
	\beq
		\vf = \rho \vE + \frac{1}{c} \vJ \times \vB
	\eeq
	as the force meter unit volume that the electromagnetic field exerts on matter.
	
	We can use the distributive property of the cross product to write
	\beq
		\vx \times \pdv{\cP}{t} - \vx \times (\grad \cdot \vT) = - \vx \times \vf = 0,
	\eeq
	where we use the notation $(\grad \cdot \vT)_i = \sum_{j=1}^3 \partial_j \Tij$, and we have used the fact that we are working with a source-free solution to write $\vf = 0$.  We are free to move the time derivative since $\vx$ represents the point at which we are evaluating the angular momentum, and is not time dependent.  Thus, we have
	\beqn \label{friend1}
		\vx \times (\grad \cdot \vT) = \pdv{}{t} (\vx \times \cP) = \pdv{\vl}{t}.
	\eeqn
	The $y$ component of this vector is
	\beq
		\pdv{\ly}{t} = z (\grad \cdot \vT)_x - x (\grad \cdot \vT)_z,
	\eeq
	where
	\begin{align*}
		(\grad \cdot \vT)_x &= \left( \pdv{T_{xx}}{x} + \pdv{T_{xy}}{y} + \pdv{T_{xz}}{z} \right) \\
		&= \frac{1}{4\pi} \left[ \pdv{}{x} \left( \Ex^2 + \Bx^2 - \frac{E^2 + B^2}{2} \right) + \pdv{}{y} (\Ex \Ey + \Bx \By) + \pdv{}{z} (\Ex \Ez + \Bx \Bz) \right].
	\end{align*}
	Note that $(\grad \cdot \vT)_y$ and $(\grad \cdot \vT)_y$ have similar forms.
	
	Integrating \refeq{friend1} over all of space,
	\beqn \label{friend2}
		\int \pdv{\ly}{t} \dcx = \int [ z (\grad \cdot \vT)_x - x (\grad \cdot \vT)_z ] \dcx.
	\eeqn
	Note that
	\beq
		\int \pdv{\vl}{t} \dcx = \limLi \intLL \intLL \intLL \pdv{\vl}{t} \dx \dy \dz,
	\eeq
	so the first term of \refeq{friend2} becomes
	\begin{align*}
		\int z (\grad \cdot \vT)_x \dcx &= \limLi \frac{1}{4\pi} \intLL \intLL \intLL z \pdv{}{x} \left( \Ex^2 + \Bx^2 - \frac{E^2 + B^2}{2} \right) \dx \dy \dz \\
		&\phantom{mmmmmmmmmm} + \limLi \frac{1}{4\pi} \intLL \intLL \intLL z \pdv{}{y} (\Ex \Ey + \Bx \By) \dx \dy \dz \\
		&\phantom{mmmmmmmmmmmmmmmmmmmm} + \limLi \frac{1}{4\pi} \intLL \intLL \intLL z \pdv{}{z} (\Ex \Ez + \Bx \Bz) \dx \dy \dz.
	\end{align*}
	For the first term of this integral, integrating by parts with respect to $x$ yields
	\beq
		\limLi \intLL \pdv{}{x} \left( \Ex^2 + \Bx^2 - \frac{E^2 + B^2}{2} \right) \dx = \limLi \bigg[ \Ex^2 + \Bx^2 - \frac{E^2 + B^2}{2} \bigLL = 0,
	\eeq
	since $\vE$ and $\vB$ vanish rapidly as $\absx \to \infty$.  For the second term,
	\beq
		\intLL \pdv{}{y} (\Ex \Ey + \Bx \By) \dy = \limLi \bigg[ \Ex \Ey + \Bx \By \bigLL = 0.
	\eeq
	For the third term,
	\beq
		\intLL z \pdv{}{z} (\Ex \Ez + \Bx \Bz) \dz = \limLi \bigg[ z (\Ex \Ez + \Bx \Bz) \bigLL - \limLi \intLL (\Ex \Ez + \Bx \Bz) \dz.
	\eeq
	Since $\vE$ and $\vB$ fall off ``rapidly,'' we assume they overtake $\absx$ as $\absx \to \infty$.  That is, $\vE, \vB \sim 1/\absx^n$ where $n > 1$.  Then
	\begin{align*}
		\limLi \bigg[ z (\Ex \Ez + \Bx \Bz) \bigLL &\sim \limLi \bigg[ \frac{1}{z^{n-1}} \bigLL = 0, &
		\limLi \intLL (\Ex \Ez + \Bx \Bz) \dz &\sim \limLi \bigg[ \frac{1}{z^{n-1}} \bigLL = 0
	\end{align*}
	
	Thus, \refeq{friend2} becomes
	\beq
		\int \pdv{\ly}{t} \dcx = 0 \implies \int \pdv{\vl}{t} \dcx = 0
	\eeq
	by symmetry.  We may move the derivative out of the integral to obtain
	\beq
		\dv{\vL}{t} = \dv{}{t} \int \vl \dcx = \int \pdv{\vl}{t} \dcx = 0,
	\eeq
	as we sought to prove. \qed
\end{solution}