\newcommand{\Px}{P_x}
\newcommand{\Py}{P_y}

\begin{statement}{Conserved quantities for a system of line vortices} \label{vort2}
\subparagraph{}
	Now consider the general case of $n$ vortices.
\end{statement}

\begin{problem} \label{6a}
	Verify that the ``total linear momentum along $x$'' and the ``total linear momentum along $y$,''
	\begin{align*}
		\Px &= \sum_{i = 1}^n \gami \yi, &
		\Py &= \sum_{i = 1}^n -\gami \xi,
	\end{align*}
	are conserved.
\end{problem}

\begin{solution}
	In order to show that $\Px$ and $\Py$ are conserved, we will show that $[H, \Px] = [H, \Py] = 0$, where $H$ is given by \refeq{ham5}.  For all $i, j$,
	\begin{align*}
		\pdv{\Px}{\xi} &= 0, &
		\pdv{\Px}{\yi} &= \gami, &
		\pdv{\Py}{\xi} &= -\gami, &
		\pdv{\Py}{\yi} &= 0,
	\end{align*}
	and
	\begin{align*}
		\pdv{H}{\xi} &= \sum_{j \neq i} - \gami \gamj \frac{\xi - \xj}{|\vri - \vrj|^2}, &
		\pdv{H}{\yi} &= \sum_{j \neq i} - \gami \gamj \frac{\yi - \yj}{|\vri - \vrj|^2}.
	\end{align*}
	Applying \refeq{poiss},
	\begin{align*}
		[H, \Px] &= \sum_{i = 1}^n \frac{1}{\gami} \left( \pdv{H}{\xi} \pdv{\Px}{\yi} - \pdv{H}{\yi} \pdv{\Px}{\xi} \right)
		= \sum_{i = 1}^n \frac{1}{\gami} \pdv{H}{\xi} \pdv{\Px}{\yi}
		= \sum_{i = 1}^n \sum_{j \neq i} -\gami \gamj \frac{\xi - \xj}{|\vri - \vrj|^2}
		= 0, \\
		[H, \Py] &= \sum_{i = 1}^n \frac{1}{\gami} \left( \pdv{H}{\xi} \pdv{\Py}{\yi} - \pdv{H}{\yi} \pdv{\Py}{\xi} \right)
		= \sum_{i = 1}^n -\frac{1}{\gami} \pdv{H}{\yi} \pdv{\Py}{\xi}
		= \sum_{i = 1}^n \sum_{j \neq i} \gami \gamj \frac{\yi - \yj}{|\vri - \vrj|^2}
		= 0,
	\end{align*}
	as desired. \qed
\end{solution}

\begin{problem}
	Verify that $[\Px, \Py]$ gives a conserved quantity.
\end{problem}

\begin{solution}
	As in \ref{6a}, we will show that $[H, [\Px, \Py]] = 0$.  Firstly, note that
	\beq
		[\Px, \Py] = \sum_{i = 1}^n \frac{1}{\gami} \left( \pdv{\Px}{\xi} \pdv{\Py}{\yi} - \pdv{\Px}{\yi} \pdv{\Py}{\xi} \right)
		= \sum_{i = 1}^n -\frac{1}{\gami} \pdv{\Px}{\yi} \pdv{\Py}{\xi}
		= \sum_{i = 1}^n \gami.
	\eeq
	It is obvious that
	\beq
		\pdv{[\Px, \Py]}{\xi} = \pdv{[\Px, \Py]}{\yi} = 0,
	\eeq
	for all $i, j$, so it follows trivially that
	\beq
		[H, [\Px, \Py]] = \sum_{i = 1}^n \frac{1}{\gami} \left( \pdv{H}{\xi} \pdv{[\Px, \Py]}{\yi} - \pdv{H}{\yi} \pdv{[\Px, \Py]}{\xi} \right) = 0
	\eeq
	as desired. \qed
\end{solution}