\newcommand{\lap}{\nabla^2}
\newcommand{\Ld}{\mathcal{L}}
\newcommand{\phis}{\phi^*}

\newcommand{\phit}{\phi_t}
\newcommand{\phix}{\phi_x}
\newcommand{\phiy}{\phi_y}

\newcommand{\phist}{\phis_t}
\newcommand{\phisx}{\phis_x}
\newcommand{\phisy}{\phis_y}

\begin{statement}{}
	Consider the real-valued Lagrangian density $\Ld$ depending on a complex-valued function $\phi(t, x, y)$:
	\beqn \label{lagr2}
		\Ld = \frac{i}{2} \left( \phis \dv{\phi}{t} - \dv{\phis}{t} \phi \right) - \nabla \phis \cdot \nabla \phi - m^2 \phis \phi,
	\eeqn
	where $^*$ is complex conjugation, and $\nabla \phi = (\pdv*{\phi}{x}, \pdv*{\phi}{y})$.  Treating $\phi$ and $\phis$ as independent objects, derive the Euler-Lagrange equations.
\end{statement}

\begin{solution}
	We will have two Euler-Lagrange equations; one for $\phi$ and one for $\phis$.  In general, they are given by
	\begin{align*}
		0 &= \pdv{\Ld}{\phi} - \dv{}{t} \pdv{\Ld}{\phit} - \dv{}{x} \pdv{\Ld}{\phix} - \dv{}{y} \pdv{\Ld}{\phiy}, &
		0 &= \pdv{\Ld}{\phis} - \dv{}{t} \pdv{\Ld}{\phist} - \dv{}{x} \pdv{\Ld}{\phisx} - \dv{}{y} \pdv{\Ld}{\phisy}.
	\end{align*}
	Expanding out $\nabla \phis \cdot \nabla \phi$, \refeq{lagr2} becomes
	\beq
		\Ld = \frac{i}{2} \left( \phis \dv{\phi}{t} - \dv{\phis}{t} \phi \right) - \pdv{\phis}{x} \pdv{\phi}{x} - \pdv{\phis}{y} \pdv{\phi}{y} - m^2 \phis \phi.
	\eeq
	Then
	\begin{align*}
		\pdv{\Ld}{\phi} &= -\frac{i}{2} \dv{\phis}{t} - m^2 \phis, &
		\pdv{\Ld}{\phit} &= \frac{i}{2} \phis, &
		\pdv{\Ld}{\phix} &= -\pdv{\phis}{x}, &
		\pdv{\Ld}{\phiy} &= -\pdv{\phis}{y}, \\
		\pdv{\Ld}{\phis} &= \frac{i}{2} \dv{\phi}{t} - m^2 \phi, &
		\pdv{\Ld}{\phist} &= -\frac{i}{2} \phi, &
		\pdv{\Ld}{\phisx} &= -\pdv{\phi}{x}, &
		\pdv{\Ld}{\phisy} &= -\pdv{\phi}{y},
	\end{align*}
	and
	\begin{align*}
		\dv{}{t} \pdv{\Ld}{\phit} &= \frac{i}{2} \dv{\phis}{t}, &
		\dv{}{x} \pdv{\Ld}{\phix} &= -\pdv[2]{\phis}{x}, &
		\dv{}{y} \pdv{\Ld}{\phiy} &= -\pdv[2]{\phis}{y}, \\
		\dv{}{t} \pdv{\Ld}{\phist} &= -\frac{i}{2} \dv{\phi}{t}, &
		\dv{}{x} \pdv{\Ld}{\phisx} &= -\pdv[2]{\phi}{x}, &
		\dv{}{y} \pdv{\Ld}{\phisy} &= -\pdv[2]{\phi}{y}.
	\end{align*}
	Then the Euler-Lagrange equations are
	\begin{align*}
		0 &= -\frac{i}{2} \dv{\phis}{t} - m^2 \phis - \frac{i}{2} \dv{\phis}{t} + \pdv[2]{\phis}{x} + \pdv[2]{\phis}{y}, &
		0 &= \frac{i}{2} \dv{\phi}{t} - m^2 \phi + \frac{i}{2} \dv{\phi}{t} + \pdv[2]{\phi}{x} + \pdv[2]{\phi}{y},
	\end{align*}
	which simplify to
	\begin{align*}
		0 &= i \dv{\phis}{t} - \lap \phis + m^2 \phis, &
		0 &= i \dv{\phi}{t} + \lap \phis - m^2 \phis.
	\end{align*}
\end{solution}