\state{Coulomb scattering (Peskin \& Schroeder 5.1)}{
	Repeat the computation of Problem 4.4, part~(c), this time using the full relativistic expression for the matrix element.  You should find, for the spin-averaged cross section,
	\eq{
		\dv{\sig}{\Omg} = \frac{\alp^2}{4 \abs{\vp}^2 \bet^2 \sin[4](\tht / 2)} \brac{ 1 - \bet^2 \sin[2](\frac{\tht}{2}) },
	}
	where $\vp$ is the electron's 3-momentum and $\bet$ its velocity.  This is the \emph{Mott formula} for Coulomb scattering of relativistic electrons.  Now derive it in a second way, by working out the cross section for electron-muon scattering, in the muon rest frame, retaining the electron mass but sending $\mmu \to \infty$.
}

\sol{
	From the solution to 2(b) of Homework~4, we know that
	\eqn{xsec1}{
		\dv{\sig}{\Omg} = \frac{\abs{\cM}^2}{16 \pi^2}.
	}
	We also know from 2(a) that
	\eq{
		i \cM = -i e \ubpp \gamm \up \cdot \tAsm(\vp' - \vp),
	}
	where the argument of $\tA$ includes only the spatial components of $p$ and $p'$ because $\Asm(x)$ is time independent~\cite[p.~129]{Peskin}.  Then
	\eq{
		-i \cMs = i e \ubp \gamm \upp \cdot \tAsm(\vp' - \vp),
	}
	so
	\eq{
		\abs{\cM}^2 = e^2 \ubpp \gamm \up \ubp \gamn \upp \tAsm(\vp' - \vp) \tAsn(\vp' - \vp).
	}
	Averaging over the spins, we want to compute~\cite[p.~132]{Peskin}
	\eq{
		\frac{1}{2} \sumssp \abs{\cM(s, s')}^2.
	}
	By (5.3) of Peskin \& Schroeder,
	\eq{
		\sums \usp \ubsp = \psl + m.
	}
	Then, writing in the spinor indices as in the equation above (5.4),
	\al{
		\frac{1}{2} \sumssp \abs{\cM}^2 &= \frac{e^2}{2} \sumssp \ubsasppp \gammsab \usbsp \ubscsp \gamnscd \usdsppp \tAsm(p' - p) \tAsn(p' - p) \\
		&= \frac{e^2}{2} \sumssp \usdsppp \ubsasppp \gammsab \usbsp \ubscsp \gamnscd \tAsm(p' - p) \tAsn(p' - p) \\
		&=\frac{e^2}{2} (\psl' + m)_{d a} \gammsab (\psl + m)_{b c} \gamnscd \tAsm(\vp' - p) \tAsn(\vp' - \vp) \\
		&= \frac{e^2}{2} \Tr[ (\psl' + m) \gamm (\psl + m) \gamn ] \tAsm(\vp' - \vp) \tAsn(\vp' - \vp).
	}
	Note that
	\aln{
		\Tr[ (\psl' + m) \gamm (\psl + m) \gamn ] &= \Tr(\psl' \gamm \psl \gamn) + \Tr(\psl' \gamm m \gamn) + \Tr(m \gamm \psl \gamn) + \Tr(m \gamm m \gamn) \notag \\
		&= \Tr(\psl' \gamm \psl \gamn) + \Tr(m \gamm m \gamn), \label{beg}
	}
	since the other two terms have an odd number of $\gam$s~\cite[p.~133]{Peskin}.  Then by Peskin \& Schroeder~(5.5),
	\eqn{}{
		\Tr(m \gamm m \gamn) = m^2 \Tr(\gamm \gamn) = 4 m^2 \gmn.
	}
	Applying $\psl = \gamm \psm$~\cite[p.~49]{Peskin},
	\eqn{end}{
		\Tr(\psl' \gamm \psl \gamn) = \psr' \pss \Tr(\gamr \gamm \gams \gamn)
		= 4 \psr' \pss (\grm \gsn - \grs \gmn + \grn \gms).
	}
	Then
	\al{
		\frac{1}{2} \sumssp \abs{\cM}^2 &= 2 e^2 \brac{ \psr' \pss (\grm \gsn - \grs \gmn + \grn \gms) + m^2 \gmn } \tAsm(\vp' - \vp) \tAsn(\vp' - \vp) \\
		&= 2 e^2 \brac{ \psr' \tAr \pss \tAs - \psr' \pr \tAsm \tAn + \psr' \tAn \pss \tAm + m^2 \tAsm \tAn } \\
		&= 2 e^2 \curly{ 2 (p' \cdot \tA) (p \cdot \tA) + [m^2 - (p' \cdot p)] (\tA \cdot \tA) },
	}
	where we  have omitted the arguments of $\tA$ for notational simplicity.  We know that for Coulomb scattering $\Asm$ has only a zeroth component, $\Ao  = Z e / 4\pi r$~\cite[p.~130]{Peskin}.  From the solution to 2(c) of Homework~4, we also know that $\tAso(\vq) = Z e / \abs{\vq}^2$.  Then
	\al{
		\frac{1}{2} \sumssp \abs{\cM}^2 &= 2 e^2 \brac{ 2 E E' \tAso^2 + (m^2 - E E' + \vp \cdot \vp') \tAso^2 } \\
		&= 2 e^2 \tAso^2 (2 E E' + m^2 - E' E + \vp \cdot \vp') \\
		&= 2 \frac{Z^2 e^4}{\abs{\vp' - \vp}^4} (E E' + m^2 + \vp \cdot \vp').
	}
	From 2(c) of Homework~4, we know
	\eq{
		\abs{\vp' - \vp}^2 = {\vp'}^2 - 2 \abs{\vp'} \abs{\vp} \cos\tht + \vp^2,
	}
	where $\tht$ is the angle between $\vp$ and $\vp'$.  Using this and taking the limit that $p = p'$,
	\eq{
		\frac{1}{2} \sumssp \abs{\cM}^2 = 2 Z^2 e^4 \frac{E E' + m^2 + \abs{\vp} \abs{\vp'} \cos\tht}{({\vp'}^2 - 2 \abs{\vp'} \abs{\vp} \cos\tht + \vp^2)^2}
		= 2 Z^2 e^4 \frac{E^2 + m^2 + \vp^2 \cos\tht}{4 \vp^4 (1 - \cos\tht)^2}
		= \frac{Z^2 e^4}{8} \frac{E^2 + m^2 + \vp^2 \cos\tht}{\vp^4 \sin[4](\tht / 2)}.
	}
	Noting that $E^2 = m^2 + p^2$,
	\eq{
		\frac{1}{2} \sumssp \abs{\cM}^2 = \frac{Z^2 e^4}{8} \frac{E^2 + E^2 - \vp^2 + \vp^2 \cos\tht}{\vp^4 \sin[4](\tht / 2)}
		= \frac{Z^2 e^4}{8} \frac{2 E^2 - \vp^2 (1 - \cos\tht)}{\vp^4 \sin[4](\tht / 2)}
		= \frac{Z^2 e^4}{4} \frac{E^2 - \vp^2 \sin[2](\tht / 2)}{\vp^4 \sin[4](\tht / 2)}.
	}
	Now using $\vp^2 = m^2 \bet^2$, $\bet = \abs{\vp} / E$, $E / m = 1$, and $\alp = e^2 / 4\pi$~\cite[p.~xxi]{Peskin},
	\eq{
		\frac{1}{2} \sumssp \abs{\cM}^2 = \frac{Z^2 e^4 E^2}{4} \frac{1 - \bet^2 \sin[2](\tht / 2)}{m^2 \bet^2 \vp^2 \sin[4](\tht / 2)}
		= \frac{Z^2 e^4 E^2}{4} \frac{1 - \bet^2 \sin[2](\tht / 2)}{m^2 \bet^2 \vp^2 \sin[4](\tht / 2)}
		= \frac{4 \pi^2 \alp^2 Z^2}{\bet^2 \vp^2 \sin[4](\tht / 2)} \brac{ 1 - \bet^2 \sin[2](\frac{\tht}{2}) }
	}
	Feeding this into Eq.~\refeq{xsec1} and setting $Z = 1$, we find
	\eq{
		\dv{\sig}{\Omg} = \frac{1}{16 \pi^2} \frac{1}{2} \sumssp \abs{\cM}^2
		= \ans{ \frac{\alp^2}{4 \bet^2 \vp^2 \sin[4](\tht / 2)} \brac{ 1 - \bet^2 \sin[2](\frac{\tht}{2}) } }
	}
	as we wanted to show. \qed
	
	The lowest-order Feynman diagram for electron-muon scattering is~\cite[p.~153]{Peskin}
	\eq{
		\centergraphics{diag/emu_t_chan} = \frac{i e^2}{q^2} \ubpp \gamm \up \ubkp \gamsm \ubk.
	}
	The corresponding squared amplitude is given the equation above Peskin \& Schroeder (5.60):
	\eq{
		\frac{1}{4} \sumspins \abs{\cM}^2 = \frac{e^4}{4 q^4} \Tr[ (\psl' + \me) \gamm (\psl + \me) \gamn ] \Tr[ (\ksl' + \mmu) \gamsm (\ksl + \mmu) \gamsn ].
%		&= \frac{8 e^4}{q^4} \brac{ (p \cdot k') (p' \cdot k) + (p \cdot k) (p' \cdot k') - \mmu^2 (p \cdot p') }
	}
	Referring to Eqs.~\refeq{beg}--\refeq{end},
	\eq{
		\frac{1}{4} \sumspins \abs{\cM}^2 = 4 \frac{e^4}{q^4} \brac{ \psr' \pss (\grm \gsn - \grs \gmn + \grn \gms) + \me^2 \gmn } \brac{ \kpa \kb (\gsam \gsbn - \gsab \gsmn + \gsan \gsmb) + \mmu^2 \gsmn }.
	}
	In the muon rest frame, $\mu = \nu = 0$.  Additionally, in sending $\mmu \to \infty$ we only keep terms f $\order{\mmu^2}$.  Then
	\al{
		\frac{1}{4} \sumspins \abs{\cM}^2 &\approx 4 \frac{e^4}{q^4} \brac{ \psr' \pss (\gro \gso - \grs \goo + \gro \gos) + \me^2 \goo } \mmu^2 \gsoo \\
		&= 4 \frac{e^4 \mmu^2}{q^4} \paren{ \ppo \po - \pps \pss + \ppo \po + \me^2 } \\
		&= 4 \frac{e^4 \mmu^2}{q^4} \paren{ E' E - E' E + \vp' \vdot \vp + E' E + \me^2 } \\
		&= 4 \frac{e^4 \mmu^2}{q^4} \paren{ E' E + \vp' \vdot \vp + \me^2 }.
	}
	From Peskin \& Schroeder~(5.69) and (5.72),
	\eq{
		q = t^2 = -2 \vp^2 (1 - \cos\tht).
	}
	Then, again taking $p' = p$ and proceeding similarly as before,
	\al{
		\frac{1}{4} \sumspins \abs{\cM}^2 &= 4 \frac{e^4 \mmu^2}{[ -2 \vp^2 (1 - \cos\tht) ]^2} \paren{ E' E + \vp' \vdot \vp + \me^2 } \\
		&= e^4 \mmu^2 \frac{E^2 + \vp^2 \cos\tht + \me^2}{\vp^4 (1 - \cos\tht)^2} \\
		&= e^4 \mmu^2 \frac{2 E^2 - \vp^2 (1 - \cos\tht)}{\vp^4 (1 - \cos\tht)^2} \\
		&= \frac{e^4 \mmu^2}{2} \frac{E^2 - \vp^2 \sin[2](\tht / 2)}{\vp^4 \sin[4](\tht / 2)} \\
		&= \frac{e^4 \mmu^2 E^2}{2} \frac{1 - \bet^2 \sin[2](\tht / 2)}{\me^2 \bet^2 \vp^2 \sin[4](\tht / 2)} \\
		&= \frac{8 \pi^2 \alp^2 \mmu^2}{\bet^2 \vp^2 \sin[4](\tht / 2)} \brac{ 1 - \bet^2 \sin[2](\frac{\tht}{2}) }.
	}
	Feeding this into Eq.~\refeq{xsec1} and sending $\mmu \to 1$, we find
	\eq{
		\dv{\sig}{\Omg} = \frac{1}{16 \pi^2} \frac{1}{4} \sumssp \abs{\cM}^2
		= \ans{ \frac{\alp^2}{4 \bet^2 \vp^2 \sin[4](\tht / 2)} \brac{ 1 - \bet^2 \sin[2](\frac{\tht}{2}) } }
	}
	as we wanted to show. \qed
}