\newcommand{\vq}{v_1}
\newcommand{\vw}{v_2}

\begin{statement}{(Jackson 11.3)}
	Show explicitly that two successive Lorentz transformations in the same direction are equivalent to a single Lorentz transformation with a velocity
	\beqn \label{given1}
		v = \frac{\vq + \vw}{1 + \vq \vw / c^2}.
	\eeqn
	This is an alternative way to derive the parallel-velocity addition law.
\end{statement}

\newcommand{\xo}{x_0}
\newcommand{\xq}{x_1}
\newcommand{\xw}{x_2}
\newcommand{\xe}{x_3}

\newcommand{\betq}{\bet_1}
\newcommand{\betw}{\bet_2}
\newcommand{\gamq}{\gam_1}
\newcommand{\gamw}{\gam_2}

\begin{solution}
	The general expression for a Lorentz transformation in the $\xq$ direction is given by Jackson~(11.16),
	\begin{align} \label{lorentz}
		c t' &= \gam (ct - \bet x), &
		x' &= \gam (x - \bet c t), &
		y' &= y, &
		z' &= z.
	\end{align}
	Define $\bet$, $\betq$, and $\betw$ by
	\begin{align*}
		\bet &= \frac{v}{c}, &
		\betq &= \frac{\vq}{c}, &
		\betw &= \frac{\vw}{c},
	\end{align*}
	and define $\gam$, $\gamq$, and $\gamw$ correspondingly.
	
	First applying the boost corresponding to $\betq$ yields
	\begin{align} \label{boost1}
		c t' &= \gamq (c t - \betq x), &
		x' &= \gamq (x - \betq c t).
	\end{align}
	Successively applying the boost corresponding to $\betw$ yields
	\begin{align} \label{boost2}
		c t'' &= \gamw (c t' - \betw x'), &
		x'' &= \gamw (x' - \betw c t').
	\end{align}
	Substituting \refeq{boost1} into \refeq{boost2} gives us
	\begin{align*}
		c t'' &= \gamq \gamw [(c t - \betq x) - \betw (x - \betq c t)]
		= \gamq \gamw [(1 + \betq \betw) c t - (\betq + \betw) x] \\
		x'' &= \gamq \gamw [(x - \betq c t) - \betw (c t - \betq x)]
		= \gamq \gamw [(1 + \betq \betw) x - (\betq + \betw) c t],
	\end{align*}
	or
	\begin{align} \label{thing1}
		c t'' &= (1 + \betq \betw) \gamq \gamw \left( c t - \frac{\betq + \betw}{1 + \betq \betw} x \right), &
		x'' &= (1 + \betq \betw) \gamq \gamw \left( x - \frac{\betq + \betw}{1 + \betq \betw} c t \right).
	\end{align}
	
	Note that
	\beq
		\frac{\betq + \betw}{1 + \betq \betw} = \frac{1}{c} \frac{\vq + \vw}{1 + \vq \vw / c^2}
		= \frac{v}{c}
		= \bet,
	\eeq
	where $v$ is defined by \refeq{given1}, and that
	\begin{align*}
		(1 + \betq \betw) \gamq \gamw &= \frac{1 + \betq \betw}{\sqrt{(1 - \betq^2) (1 - \betw^2)}}
		= \sqrt{\frac{(1 + \betq \betw)^2}{(1 - \betq^2) (1 - \betw^2)}}
		= \sqrt{\frac{(1 + \betq \betw)^2}{1 - \betq^2 - \betw^2 + \betq^2 \betw^2}} \\
		&= \sqrt{\frac{(1 + \betq \betw)^2}{1 + 2 \betq \betw + \betq^2 \betw^2 - (\betq^2 + 2 \betq \betw + \betw^2)}}
		= \sqrt{\frac{(1 + \betq \betw)^2}{(1 + \betq \betw)^2 - (\betq + \betw)^2}} \\
		&= \sqrt{1 - \left( \frac{\betq + \betw}{1 + \betq \betw} \right)^2}^{\,-1}
		= \sqrt{1 - \bet^2}^{\,-1}
		= \gam.
	\end{align*}
	Then \refeq{thing1} becomes
	\begin{align*}
		\xo'' &= \gam \left( \xo - \bet \xq \right), &
		\xq'' &= \gam \left( \xq - \bet \xo \right),
	\end{align*}
	which is a single Lorentz transformation with velocity $v$, as we wanted to show. \qed
\end{solution}