\newcommand{\phio}{\phi_0}
\newcommand{\cE}{\mathcal{E}}
\newcommand{\cEint}{\cE_\text{int}}
\newcommand{\vP}{\vb{P}}
\newcommand{\evP}{\ev{\vP}}
\newcommand{\divP}{\div{\evP}}

\newcommand{\tfor}{\quad \text{for }}
\newcommand{\Ytotv}{Y_{2 0}\tv}

\begin{statement}{}
	A dielectric ball of radius $R$ and dielectric constant $\eps$ is placed in the external electrostatic potential $\phio = \alp (2z^2 - x^2 - y^2)$ where $\alp$ is a constant, with the center of the ball at $\vx = 0$.
\end{statement}

\begin{problem}
	Find the total electrostatic potential $\phi$ everywhere.
	
	Hint: It is useful to note that the external potential is proportional to $r^2 \, \Ytotv$.  This should allow you to determine/guess the form of the total potential inside and outside the dielectric up to unknown constants, which can then be determined by matching.
\end{problem}

\begin{solution}
	Firstly, note that
	\beq
		\Ytotv = \frac{1}{4} \sqrt{\frac{5}{\pi}} (3 \cos^2\tht - 1),
	\eeq
	and
	\beq
		\phio = \alp r^2 (3 \cos^2\tht - 1) = 4 \alp r^2 \sqrt{\frac{\pi}{5}} \Ytotv \equiv \beta r^2 \, \Ytotv,
	\eeq
	where we have defined $\beta \equiv 4 \alp \sqrt{\pi/5}$.

	As in problem~\ref{1}, $\rhof = 0$ so we need to solve Lapace's equation \refeq{poissdie}, which has general solutions given by \refeq{lapsol}.  In the region $r < R$, we must have $\Blm = 0$ because $1/r^{l+1}$ is undefined at the origin.  In the region $r > R$, we may invoke the boundary condition at infinity:
	\beq
		\phi(r > R, \tht, \vph) \to \phio = \beta r^2 \, \Ytotv,
	\eeq
	where we note that $\evphi = \phi$ for $r > R$.  This implies that the only nonzero $\Alm$ here is $A_{2 0} = \beta$.  Thus we have
	\beq
		\evphi\!(r, \tht, \vph) = \begin{cases}
			\dsum_{l,m} \Alm r^l \, \Ylm\tv & \tif r \leq R, \\[2ex]
			\beta r^2 \, \Ytotv + \dsum_{l,m} \dfrac{\Blm}{r^{l+1}} \, \Ylm\tv & \tif r \geq R.
		\end{cases}
	\eeq
	
	To solve for the remaining coefficients, we invoke the boundary conditions at $r = R$.  Firstly, $\evphi$ must be continuous at the boundary.  This gives us
	\beq
		\evphi\!(R, \tht, \vph) = \sum_{l,m} \Alm R^l \, \Ylm\tv = \beta R^2 \, \Ytotv + \sum_{l,m} \dfrac{\Blm}{R^{l+1}} \, \Ylm\tv,
	\eeq
	so
	\begin{align} \label{c1}
		A_{2 0} &= \beta + \dfrac{B_{2 0}}{R^{5}}, &
		\Alm &= \frac{\Blm}{R^{l+3}} \tfor (l,m) \neq (2,0).
	\end{align}
	
	Secondly, we require that $\nh \cdot \evD$ is also continuous at the boundary, where $\evD$ is defined in \refeq{D}.  Here $\nh = \rh$, so we are only concerned with the $r$ component of $\evE$.  Applying $\evE = -\grad\!\evphi$, we have
	\beq
		\evEr\!(r, \tht, \phi) = \begin{cases}
			\dsum_{l,m} \Alm l r^{l-1} \, \Ylm\tv & \tif r \leq R, \\[2ex]
			2 \beta r \, \Ytotv - \dsum_{l,m} (l + 1) \dfrac{\Blm}{r^{l+2}} \, \Ylm\tv & \tif r \geq R.
		\end{cases}
	\eeq
	Then we need to satisfy
	\beq
		\rh \cdot \evD\!(R, \tht, \vph) = \eps \sum_{l,m} \Alm l R^{l-1} \, \Ylm\tv = 2 \beta R \, \Ytotv - \sum_{l,m} (l + 1) \dfrac{\Blm}{R^{l+2}} \, \Ylm\tv,
	\eeq
	which stipulates
	\begin{align} \label{c2}
		A_{2 0} &= \frac{1}{\eps} \left( \beta - \frac{3}{2} \frac{B_{2 0}}{R^{5}} \right), &
		\Alm &= -\frac{1}{\eps} \frac{(l + 1)}{l} \frac{\Blm}{R^{2l+1}} \tfor (l,m) \neq (2,0).
	\end{align}
	Eliminating $\Blm$ from \refeq{c1} and \refeq{c2}, we obtain
	\begin{align*}
		A_{2 0} &= \frac{5 \beta}{2\eps + 3}, &
		\Alm &= 0 \tfor (l,m) \neq (2,0),
	\end{align*}
	and substituting back into \refeq{c1} yields
	\begin{align*}
		B_{2 0} &= 2 \beta R^5 \frac{1 - \eps}{2\eps + 3}, &
		\Blm &= 0 \tfor (l,m) \neq (2,0).
	\end{align*}
	
	Finally, the total electrostatic potential everywhere is
	\beqn \label{phisph}
		\evphi\!(r, \tht, \vph) = \alp (3 \cos^2\tht - 1) r^2 \times \begin{cases}
			\dfrac{5}{2\eps + 3} & \tif r \leq R, \\[2ex]
			1 + 2 \dfrac{1 - \eps}{2\eps + 3} \dfrac{R^5}{r^5} & \tif r \geq R,
		\end{cases}
	\eeqn
	or, in Cartesian coordinates,
	\beq
		\evphi\!(x, y, z) = \alp (2z^2 - x^2 - y^2) \times \begin{cases}
			\dfrac{5}{2\eps + 3} & \tif r \leq R, \\[2ex]
			1 + 2 \dfrac{1 - \eps}{2\eps + 3} \dfrac{R^5}{\sqrt{x^2 + y^2 + z^2}} & \tif r \geq R.
		\end{cases}
	\eeq
\end{solution}
\vfix



\newcommand{\sE}{\mathscr{E}}
\newcommand{\sEint}{\sE_\text{int}}
\newcommand{\vEo}{\vE_0}
\newcommand{\thh}{\boldsymbol{\hat{\tht}}}
\newcommand{\phh}{\boldsymbol{\hat{\vph}}}
\newcommand{\sint}{\sin\tht}
\newcommand{\Eth}{E_\tht}
\newcommand{\Eph}{E_\vph}
\newcommand{\evEth}{\ev{\Eth}}
\newcommand{\evEph}{\ev{\Eph}}
\newcommand{\Eo}{E_0}
\newcommand{\Eor}{{\Eo}_r}
\newcommand{\Eoth}{{\Eo}_\tht}
\newcommand{\Eoph}{{\Eo}_\vph}

\newcommand{\evPr}{\ev{P_r}}
\newcommand{\evPth}{\ev{P_\tht}}
\newcommand{\evPph}{\ev{P_\vph}}
\newcommand{\dph}{\dd{\vph}}
\newcommand{\intRi}{\int_R^\infty}
\newcommand{\intoR}{\int_0^R}

\begin{problem}
	Calculate the interaction energy between the field produced by the dielectric and the external field.  Assume that the potential arises from ``distant charges'' so that the formula for $\cEint$ given in class and the notes can be used.
\end{problem}

\begin{solution}
	Equation~(3.34) in the lectures notes gives the interaction energy:
	\beq
		\sEint = \int (\evrhof \!\phio - \evP \cdot \vEo) \dcx,
	\eeq
	where $\vEo$ is the electric field due to the external potential $\phio$.  Again, $\rhof = 0$.  For our assumption of a linear, homogeneous, and isotropic dielectric,
	\beq
		\evP = \chi \!\evE
	\eeq
	by Eq.~(3.19), where
	\beq
		\eps = 1 + 4\pi \chi
	\eeq
	from Eq.~(3.21).
	
	The gradient in spherical coordinates is
	\beqn \label{grad}
		\grad = \pdv{}{r} \,\rh + \frac{1}{r} \pdv{}{\tht} \,\thh + \frac{1}{r \sint} \pdv{}{\vph} \, \phh.
	\eeqn
	Differentiating \refeq{phisph} for $r \leq R$,
	\begin{align} \label{Ein}
		\evEr &= 2 \alp \frac{5}{2\eps + 3} r (3 \cos^2\tht - 1), &
		\evEth &= -6 \alp \frac{5}{2\eps + 3} r \cost \sint, &
		\evEph &= 0.
	\end{align}
	For the external field,
	\begin{align} \label{E0}
		\Eor &= 2 \alp r (3 \cos^2\tht - 1), &
		\Eoth &= -6 \alp r \cost \sint, &
		\Eoph &= 0.
	\end{align}
	Note that $\evP = (\eps - 1) \!\evE\! / 4 \pi$, so
	\beq
		\evP \cdot \vEo = 4 \alp^2 \frac{\eps - 1}{4\pi} \frac{5}{2\eps + 3} r^2 \left[ (3 \cos^2\tht - 1)^2 + 9 \cos^2\tht \sin^2\tht \right]
	\eeq
	Then
	\begin{align*}
		\sEint &= -\int \evP \cdot \vEo \dcx
		= 4 \alp^2 \frac{1 - \eps}{4\pi} \frac{5}{2\eps + 3} \intotp \dph \intono (3 \cos^2\tht + 1) \dct \intoR r^4 \dr \\
		&= 4 \alp^2 \frac{1 - \eps}{4\pi} \frac{5}{2\eps + 3} \bigg[ \vph \bigg]_0^{2\pi} \bigg[ \cos^3\tht + \cost \bigg]_{-1}^1 \left[ \frac{r^5}{5} \right]_0^R
		= 4 \alp^2 \frac{1 - \eps}{4\pi} \frac{5}{2\eps + 3} (2\pi) (4) \frac{R^5}{5}
		= 8 \alp^2 \frac{1 - \eps}{2\eps + 3} R^5.
	\end{align*}
\end{solution}
\vfix



\newcommand{\vF}{\vb{F}}

\begin{problem}
	Calculate the total force needed to hold the dielectric ball in place.
\end{problem}

\begin{solution}
	Equation~(3.26) in the lecture notes gives the total force on a dielectric:
	\beq
		\vF = \int [\evrhof\! \vEo + (\evP \cdot \grad) \vEo] \dcx.
	\eeq
	In electrostatics, there is no contribution from the dielectric's self field, and here $\rhof = 0$.  To find the force needed to hold the ball in place, we will need to insert a minus sign.
	
	From \refeq{Ein} and \refeq{grad}, we have
	\beq
		\evP \cdot \grad = 2\alp \frac{\eps - 1}{4\pi} \frac{5}{2\eps + 3} \left[ r (3 \cos^2\tht - 1) \pdv{}{r} - 3 \cost \sint \pdv{}{\tht} \right].
	\eeq
	From \refeq{E0}, note that
	\begin{align*}
		\pdv{\vEo}{r} &= \pdv{}{r} \left[ 2 \alp r (3 \cos^2\tht - 1) \,\rh - 6 \alp r \cost \sint \,\thh \right]
		= 2 \alp \left[ (3 \cos^2\tht - 1) \,\rh - 3 \cost \sint \,\thh \right], \\[2ex]
		\pdv{\vEo}{\tht} &= \pdv{}{\tht} \left[ \alp r (3 \cos2\tht + 1) \,\rh - 3 \alp r \sin2\tht \,\thh \right]
		= -6\alp r (\sin2\tht \,\rh + \cos2\tht \,\thh) \\
		&= -6 \alp r \left[ 2 \cost \sint \,\rh + (\cos^2\tht - \sin^2\tht) \,\thh \right].
	\end{align*}
	Then
	\begin{align*}
		(\evP \cdot \grad) \vEo &= 2\alp \frac{\eps - 1}{4\pi} \frac{5}{2\eps + 3} \left[ r (3 \cos^2\tht - 1) \pdv{\vEo}{r} - 3 \cost \sint \pdv{\vEo}{\tht} \right] \\
		&= 4\alp^2  \frac{\eps - 1}{4\pi} \frac{5}{2\eps + 3} r \!\left[ (3 \cos^2\tht - 1) \!\left( (3 \cos^2\tht - 1) \,\rh - 3 \cost \sint \,\thh \right)\! \right. \\
		&\phantom{mmmmmmmmmmmmmmmmmmmmmmm} \left. + 9 \cost \sint \!\left( 2 \cost \sint \,\rh + (\cos^2\tht - \sin^2\tht) \,\thh \right) \right] \\
		&= 4\alp^2  \frac{\eps - 1}{4\pi} \frac{5}{2\eps + 3} r \!\left[ \left( (3 \cos^2\tht - 1)^2 - 18 \cos^2\tht \sin^2\tht \right) \rh \right. \\
		&\phantom{mmmmmmmmmmmmmmmmmmmmmmm} \left. + 3 \cost \sint \left( 1 - 3\cos^2\tht + 3 (\cos^2\tht - \sin^2\tht) \right) \thh \right] \\
		&= 4\alp^2  \frac{\eps - 1}{4\pi} \frac{5}{2\eps + 3} r \!\left[ (-9\cos^4\tht + 12\cos^2\tht + 1) \,\rh + 3 \cost (-3\sin^2\tht + \sint) \,\thh \right],
	\end{align*}
	and the integral becomes
	\begin{align*}
		\vF &= -\int (\evP \cdot \grad) \vEo \dcx \\
		&= -4\alp^2  \frac{\eps - 1}{4\pi} \frac{5}{2\eps + 3} \intotp \intono \intoR r^3 \!\left[ (-9\cos^4\tht + 12\cos^2\tht + 1) \,\rh + 3 \cost (-3\sin^2\tht + \sint) \,\thh \right] \dr \dct \dph \\
		&= -4\alp^2 \frac{\eps - 1}{4\pi} \frac{5}{2\eps + 3} \intotp \dph \intono \left[ (-9\cos^4\tht + 12\cos^2\tht + 1) \,\rh + 3 \cost (-3\sin^2\tht + \sint) \,\thh \right] \dct \intoR r^3 \dr.
	\end{align*}
	For the second integral, note that
	\beq
		\intono \cost (-3\sin^2\tht + \sint) \dct
		= \int_0^\pi \cost \sint (-3\sin^2\tht + \sint) \dd{\tht}
		= \int_0^0 (-3\sin^3\tht + \sin^3\tht) \dd{(\sint)}
		= 0.
	\eeq
	Then we have
	\begin{align*}
		\vF &= -4\alp^2 \frac{\eps - 1}{4\pi} \frac{5}{2\eps + 3} \bigg[ \vph \bigg]_0^{2\pi} \left[ -\frac{9}{5} \cos^5\tht + 4 \cos^3\tht + \cost \right]_{-1}^1 \left[ \frac{r^4}{4} \right]_0^R \rh
		= -4\alp^2 \frac{\eps - 1}{4\pi} \frac{5}{2\eps + 3} (2\pi) \left( \frac{32}{5} \right) \frac{R^4}{4} \,\rh \\
		&= 16 \alp^2 \frac{1 - \eps}{2\eps + 3} R^4 \,\rh.
	\end{align*}
\end{solution}
\vfix