\documentclass[11pt]{article}
\usepackage{homework}

\classname{361}
\homeworknum{1}




\DeclareSIUnit{\mole}{mol}

\begin{document}

\input{definitions}
\input{probdefs}

\input{Problem1}

\input{Problem2}

\input{Problem3}

\input{Problem4}




\clearpage

\state{Acoustic and optic phonons in the diatomic chain}{
	In the diatomic chain, we take the unit cell to be of length $a$, and take $\xA$ and $\xB$ to be the coordinates of the A and B atoms within the unit cell.  Hence, in the $n$th cell,
	\al{
		\rnA &= n a + \xA; &
		\rnB &= n a + \xB
	}
	\vfix
}

\prob{}{
	In the equations of motion Eq.~(2.30), look for solutions of the form
	\eqn{5a}{
		\unalp = \ealpq \exp( i [ q \rnalp - \omgq t ] ) + \ealpsq \exp( i [-q \rnalp + \omgq t] )
	}
	where $\alp = A$ or $B$, and $\ealp$ are complex numbers that give the amplitude and phase of the oscillation of the two atoms.
	
	Separating out the terms that have the same time dependence, show that (for equal masses, ${\mA = \mB = m}$)
	\al{
		m \omgsq \eAq &= \DAAq \eAq + \DABq \eBq, \\
		m \omgsq \eBq &= \DBAq \eAq + \DBBq \eBq,
	}
	where
	\al{
		\DAAq &= \DBBq = K + K', \\
		-\DABq &= K \exp( i q [ \rnB - \rnA ] ) + K' \exp( i q [ \rnmqB - \rnA ] ), \\
		-\DBAq &= K \exp( i q [ \rnA - \rnB ] ) + K' \exp( i q [ \rnpqA - \rnB ] ).
	}
	Check that $\DAB = \DsBA$.
}

\sol{
	Equation~(2.30) is
	\aln{ \label{thing5a}
		\mA \pdv[2]{\unA}{t} &= K (\unB - \unA) + K' (\unmqB - \unA), &
		\mB \pdv[2]{\unB}{t} &= K' (\unpqA - \unB) + K (\unA - \unB).
	}
	Note that
	\al{
		\pdv[2]{\unalp}{t} &= \pdv{t}\{ -i \omgq \ealpq \exp( i [ q \rnalp - \omgq t ] ) + i \omgq \ealpsq \exp( i [-q \rnalp + \omgq t] ) \} \\
		&= -\omgsq \{ \ealpq \exp( i [ q \rnalp - \omgq t ] ) + \ealpsq \exp( i [-q \rnalp + \omgq t] ) \} \\
		&= -\omgsq \unalp,
	}
	so the first of Eq.~\refeq{5a} can be written
	\al{
		[ K + K' - \mA \omgsq ] \unA &= K \unB + K' \unmqB, \\[1ex]
		&= K \eBq e^{i q \rnB} e^{-i \omgq t} + K \eBsq e^{-i q \rnB} e^{i \omgq t} + K' \eBq e^{i q \rnmqB} e^{-i \omgq t} \\
		&\hspace{5em} \phantom{=\ } + K' \eBsq e^{-i q \rnmqB} e^{i \omgq t} \\[1ex]
		&= K \eBq e^{i q [ na + \xB ]} e^{-i \omgq t} + K' \eBq e^{i q [ (n - 1) a + \xB ]} e^{-i \omgq t} + K \eBsq e^{-i q [ na + \xB ]} e^{i \omgq t} \\
		&\phantom{=\ } + K' \eBsq e^{-i q [ (n - 1) a + \xB ]} e^{i \omgq t} \\[1ex]
		&= (K + e^{-i q a} K') \eBq e^{i q (na + \xB)} e^{-i \omgq t} + (K + e^{-i q a} K') \eBsq e^{-i q (na + \xB)} e^{i \omgq t} \\[1ex]
		&= (K + e^{-i q a} K') \unB.
	}
	Generalizing this, we have
	\al{
		[ K + K' - \mA \omgsq ] \unA &= (K + e^{-i q a} K') \unB, &
		[ K + K' - \mB \omgsq ] \unB &= (K + e^{i q a} K') \unA.
	}
	
	Collecting terms of like time dependence gives us
	\aln{
		[ K + K' - m \omgsq ] \eAq e^{i q \rnA} &= (K + e^{-i q a} K') \eBq e^{i q \rnB}, \label{thing5.a1} \\
		[ K + K' - m \omgsq ] \eBq e^{i q \rnB} &= (K + e^{i q a} K') \eAq e^{i q \rnA}, \label{thing5.a2}
	}
	for $e^{-i \omg t}$, and
	\aln{
		[ K + K' - m \omgsq ] \eAsq e^{-i q \rnA} &= (K + e^{-i q a} K') \eBsq e^{-i q \rnB}, \label{thing5.a3} \\
		[ K + K' - m \omgsq ] \eBsq e^{i q \rnB} &= (K + e^{-i q a} K') \eAsq e^{-i q \rnA}. \label{thing5.a4}
	}
	for $e^{i \omg t}$.
	
	Rearranging Eqs.~\refeq{thing5.a1} and \refeq{thing5.a2}
}



%\prob{}{
%	The $2 \times 2$ matrix equation can have a nontrivial solution if the determinant vanishes:
%	\eq{
%		\mqty| 	\DAAq - m \omgsq & \DABq \\
%				\DBAq & \DBBq - m \omgsq |
%		= 0.
%	}
%	Hence show that the frequencies of the modes are given by
%	\eq{
%		m \omgsq = K + K' \pm \sqrt{ (K + K')^2 - 4 K K' \sin[2]( \frac{q a}{2} ) }.
%	}
%	\vfix
%}



%\prob{}{
%	Sketch the dispersion relations when $K / K' =  2$.  Discuss what happens if $K = K'$.
%}




\clearpage

\input{Problem6}




\makebib

\end{document}
